w64x4/proof/Fp_w64x4_extract.ec
@@ -1,13 +1,13 @@
 require import AllCore IntDiv CoreMap List Distr.
-require import JModel.
+ require import JModel.
 
-require import Array4.
-require import WArray32.
+require import Array4 Array8 Array16.
+(* require import WArray32 WArray64 WArray128. *)
 
 
 
 module M = {
-  proc bn_subc (a:W64.t Array4.t, b:W64.t Array4.t) : bool * W64.t Array4.t = {
+  proc dbn_subc (a:W64.t Array8.t, b:W64.t Array8.t) : bool * W64.t Array8.t = {
     var aux: int;
     
     var cf:bool;
@@ -20,7 +20,7 @@ module M = {
     (cf, x1) <- subc_64 x1 x2 false;
     a.[0] <- x1;
     i <- 1;
-    while (i < 4) {
+    while (i < 8) {
       x1 <- a.[i];
       x2 <- b.[i];
       (cf, x1) <- subc_64 x1 x2 cf;
@@ -30,212 +30,349 @@ module M = {
     return (cf, a);
   }
   
-  proc bn_addc (a:W64.t Array4.t, b:W64.t Array4.t) : bool * W64.t Array4.t = {
+  proc dbn_copy (a:W64.t Array8.t) : W64.t Array8.t = {
     var aux: int;
     
+    var r:W64.t Array8.t;
+    var i:int;
+    var t:W64.t;
+    r <- witness;
+    i <- 0;
+    while (i < 8) {
+      t <- a.[i];
+      r.[i] <- t;
+      i <- i + 1;
+    }
+    return (r);
+  }
+  
+  proc mul1 (a:W64.t, b:W64.t Array4.t) : W64.t * bool * bool *
+                                          W64.t Array8.t = {
+    var aux: int;
+    
+    var _zero:W64.t;
+    var of_0:bool;
     var cf:bool;
+    var r:W64.t Array8.t;
     var x1:W64.t;
     var x2:W64.t;
     var i:int;
-    
-    x1 <- a.[0];
+    var lo:W64.t;
+    var  _0:bool;
+    var  _1:bool;
+    var  _2:bool;
+    r <- witness;
+    (of_0, cf,  _0,  _1,  _2, _zero) <- set0_64 ;
+    x1 <- a;
     x2 <- b.[0];
-    (cf, x1) <- addc_64 x1 x2 false;
-    a.[0] <- x1;
+    (x1, x2) <- MULX_64 x1 x2;
+    r.[1] <- x1;
+    r.[0] <- x2;
     i <- 1;
     while (i < 4) {
-      x1 <- a.[i];
+      x1 <- a;
       x2 <- b.[i];
-      (cf, x1) <- addc_64 x1 x2 cf;
-      a.[i] <- x1;
+      (x1, x2) <- MULX_64 x1 x2;
+      r.[(i + 1)] <- x1;
+      lo <- x2;
+      x1 <- r.[i];
+      x2 <- lo;
+      (cf, x1) <- ADCX_64 x1 x2 cf;
+      r.[i] <- x1;
       i <- i + 1;
     }
-    return (cf, a);
+    x1 <- r.[4];
+    (cf, x1) <- ADCX_64 x1 _zero cf;
+    r.[4] <- x1;
+    return (_zero, of_0, cf, r);
   }
   
-  proc ith_bit64 (k:W64.t, ctr:W64.t) : W64.t = {
-    
-    var bit:W64.t;
-    var p:W64.t;
-    
-    bit <- k;
-    p <- ctr;
-    p <- (p `&` (W64.of_int 63));
-    bit <- (bit `>>` (truncateu8 p));
-    bit <- (bit `&` (W64.of_int 1));
-    return (bit);
-  }
-  
-  proc ith_bit (kk:W64.t Array4.t, ctr:W64.t) : W64.t = {
-    
-    var bit:W64.t;
-    var ctr2:W64.t;
-    var ctr3:W64.t;
-    var c1:W64.t;
-    var c2:W64.t;
-    var r:W64.t;
-    
-    ctr2 <- ctr;
-    ctr3 <- ctr;
-    c1 <- (ctr2 `>>` (W8.of_int 6));
-    c2 <- (ctr3 `&` (W64.of_int 63));
-    r <- kk.[(W64.to_uint c1)];
-    bit <@ ith_bit64 (r, c2);
-    return (bit);
-  }
-  
-  proc swapr (x:W64.t Array4.t, y:W64.t Array4.t, swap_0:W64.t) : W64.t Array4.t *
-                                                                  W64.t Array4.t = {
+  proc mul1acc (k:int, a:W64.t, b:W64.t Array4.t, r:W64.t Array8.t,
+                _zero:W64.t, of_0:bool, cf:bool) : W64.t * bool * bool *
+                                                   W64.t Array8.t = {
     var aux: int;
     
-    var mask:W64.t;
+    var x1:W64.t;
     var i:int;
-    var tmp1:W64.t;
-    var tmp2:W64.t;
+    var x2:W64.t;
+    var hi:W64.t;
+    var lo:W64.t;
     
-    mask <- (swap_0 * (W64.of_int 18446744073709551615));
+    aux <- (4 - 1);
     i <- 0;
-    while (i < 4) {
-      tmp1 <- x.[i];
-      tmp1 <- (tmp1 `^` y.[i]);
-      tmp1 <- (tmp1 `&` mask);
-      x.[i] <- (x.[i] `^` tmp1);
-      tmp2 <- y.[i];
-      tmp2 <- (tmp2 `^` tmp1);
-      y.[i] <- tmp2;
+    while (i < aux) {
+      x1 <- a;
+      x2 <- b.[i];
+      (x1, x2) <- MULX_64 x1 x2;
+      hi <- x1;
+      lo <- x2;
+      x1 <- r.[(k + i)];
+      (of_0, x1) <- ADOX_64 x1 lo of_0;
+      r.[(k + i)] <- x1;
+      x1 <- r.[((k + i) + 1)];
+      (cf, x1) <- ADCX_64 x1 hi cf;
+      r.[((k + i) + 1)] <- x1;
       i <- i + 1;
     }
-    return (x, y);
+    x1 <- a;
+    x2 <- b.[(4 - 1)];
+    (x1, x2) <- MULX_64 x1 x2;
+    r.[(4 + k)] <- x1;
+    lo <- x2;
+    x1 <- r.[((4 + k) - 1)];
+    (of_0, x1) <- ADOX_64 x1 lo of_0;
+    r.[((4 + k) - 1)] <- x1;
+    x1 <- r.[(4 + k)];
+    (cf, x1) <- ADCX_64 x1 _zero cf;
+    r.[(4 + k)] <- x1;
+    x1 <- r.[(4 + k)];
+    (of_0, x1) <- ADOX_64 x1 _zero of_0;
+    r.[(4 + k)] <- x1;
+    return (_zero, of_0, cf, r);
   }
   
-  proc cminusP (p:W64.t Array4.t, x:W64.t Array4.t) : W64.t Array4.t = {
+  proc bn_muln (a:W64.t Array4.t, b:W64.t Array4.t) : W64.t * bool * bool *
+                                                      W64.t Array8.t = {
+    var aux: int;
     
-    var t:W64.t Array4.t;
-    var z:W64.t Array4.t;
+    var _zero:W64.t;
+    var of_0:bool;
     var cf:bool;
+    var r:W64.t Array8.t;
+    var ai:W64.t;
+    var i:int;
+    r <- witness;
+    ai <- a.[0];
+    (_zero, of_0, cf, r) <@ mul1 (ai, b);
+    i <- 1;
+    while (i < 4) {
+      ai <- a.[i];
+      (_zero, of_0, cf, r) <@ mul1acc (i, ai, b, r, _zero, of_0, cf);
+      i <- i + 1;
+    }
+    return (_zero, of_0, cf, r);
+  }
+  
+  proc dmul1 (a:W64.t, b:W64.t Array8.t) : W64.t * bool * bool *
+                                           W64.t Array16.t = {
+    var aux: int;
+    
+    var _zero:W64.t;
+    var of_0:bool;
+    var cf:bool;
+    var r:W64.t Array16.t;
+    var x1:W64.t;
+    var x2:W64.t;
+    var i:int;
+    var lo:W64.t;
+    var  _0:bool;
+    var  _1:bool;
+    var  _2:bool;
+    r <- witness;
+    (of_0, cf,  _0,  _1,  _2, _zero) <- set0_64 ;
+    x1 <- a;
+    x2 <- b.[0];
+    (x1, x2) <- MULX_64 x1 x2;
+    r.[1] <- x1;
+    r.[0] <- x2;
+    i <- 1;
+    while (i < 8) {
+      x1 <- a;
+      x2 <- b.[i];
+      (x1, x2) <- MULX_64 x1 x2;
+      r.[(i + 1)] <- x1;
+      lo <- x2;
+      x1 <- r.[i];
+      x2 <- lo;
+      (cf, x1) <- ADCX_64 x1 x2 cf;
+      r.[i] <- x1;
+      i <- i + 1;
+    }
+    x1 <- r.[8];
+    (cf, x1) <- ADCX_64 x1 _zero cf;
+    r.[8] <- x1;
+    return (_zero, of_0, cf, r);
+  }
+  
+  proc dmul1acc (k:int, a:W64.t, b:W64.t Array8.t, r:W64.t Array16.t,
+                 _zero:W64.t, of_0:bool, cf:bool) : W64.t * bool * bool *
+                                                    W64.t Array16.t = {
+    var aux: int;
+    
+    var x1:W64.t;
+    var i:int;
+    var x2:W64.t;
+    var hi:W64.t;
+    var lo:W64.t;
+    
+    aux <- (8 - 1);
+    i <- 0;
+    while (i < aux) {
+      x1 <- a;
+      x2 <- b.[i];
+      (x1, x2) <- MULX_64 x1 x2;
+      hi <- x1;
+      lo <- x2;
+      x1 <- r.[(k + i)];
+      (of_0, x1) <- ADOX_64 x1 lo of_0;
+      r.[(k + i)] <- x1;
+      x1 <- r.[((k + i) + 1)];
+      (cf, x1) <- ADCX_64 x1 hi cf;
+      r.[((k + i) + 1)] <- x1;
+      i <- i + 1;
+    }
+    x1 <- a;
+    x2 <- b.[(8 - 1)];
+    (x1, x2) <- MULX_64 x1 x2;
+    r.[(8 + k)] <- x1;
+    lo <- x2;
+    x1 <- r.[((8 + k) - 1)];
+    (of_0, x1) <- ADOX_64 x1 lo of_0;
+    r.[((8 + k) - 1)] <- x1;
+    x1 <- r.[(8 + k)];
+    (cf, x1) <- ADCX_64 x1 _zero cf;
+    r.[(8 + k)] <- x1;
+    x1 <- r.[(8 + k)];
+    (of_0, x1) <- ADOX_64 x1 _zero of_0;
+    r.[(8 + k)] <- x1;
+    return (_zero, of_0, cf, r);
+  }
+  
+  proc dbn_muln (a:W64.t Array8.t, b:W64.t Array8.t) : W64.t * bool * bool *
+                                                       W64.t Array16.t = {
+    var aux: int;
+    
+    var _zero:W64.t;
+    var of_0:bool;
+    var cf:bool;
+    var r:W64.t Array16.t;
+    var ai:W64.t;
+    var i:int;
+    r <- witness;
+    ai <- a.[0];
+    (_zero, of_0, cf, r) <@ dmul1 (ai, b);
+    i <- 1;
+    while (i < 8) {
+      ai <- a.[i];
+      (_zero, of_0, cf, r) <@ dmul1acc (i, ai, b, r, _zero, of_0, cf);
+      i <- i + 1;
+    }
+    return (_zero, of_0, cf, r);
+  }
+  
+  proc dcminusP (p:W64.t Array8.t, x:W64.t Array8.t) : W64.t Array8.t = {
+    var aux: int;
+    
+    var z:W64.t Array8.t;
+    var cf:bool;
+    var i:int;
     var r1:W64.t;
     var r2:W64.t;
-    t <- witness;
     z <- witness;
-    z.[0] <- x.[0];
-    z.[1] <- x.[1];
-    z.[2] <- x.[2];
-    z.[3] <- x.[3];
-    (cf, t) <@ bn_subc (z, p);
-    r1 <- t.[0];
-    r2 <- x.[0];
-    r1 <- (cf ? r2 : r1);
-    t.[0] <- r1;
-    r1 <- t.[1];
-    r2 <- x.[1];
-    r1 <- (cf ? r2 : r1);
-    t.[1] <- r1;
-    r1 <- t.[2];
-    r2 <- x.[2];
-    r1 <- (cf ? r2 : r1);
-    t.[2] <- r1;
-    r1 <- t.[3];
-    r2 <- x.[3];
-    r1 <- (cf ? r2 : r1);
-    t.[3] <- r1;
-    return (t);
-  }
-  
-  proc addm (p:W64.t Array4.t, a:W64.t Array4.t, b:W64.t Array4.t) : 
-  W64.t Array4.t = {
-    
-    var f:W64.t Array4.t;
-    var z:W64.t Array4.t;
-    var  _0:bool;
-    f <- witness;
-    z <- witness;
-    ( _0, f) <@ bn_addc (a, b);
-    z.[0] <- f.[0];
-    z.[1] <- f.[1];
-    z.[2] <- f.[2];
-    z.[3] <- f.[3];
-    f <@ cminusP (p, z);
-    return (f);
-  }
-  
-  proc mulm (m:W64.t Array4.t, x:W64.t Array4.t, n:W64.t Array4.t) : 
-  W64.t Array4.t = {
-    
-    var x1:W64.t Array4.t;
-    var ctr:W64.t;
-    var x2:W64.t Array4.t;
-    var d:W64.t;
-    var x3:W64.t Array4.t;
-    var x4:W64.t Array4.t;
-    var p:W64.t;
-    var lbit:W64.t;
-    var t1:W64.t;
-    var t2:W64.t;
-    var q:W64.t;
-    var par:W64.t;
-    var cbit:W64.t;
-    x1 <- witness;
-    x2 <- witness;
-    x3 <- witness;
-    x4 <- witness;
-    ctr <- (W64.of_int ((4 * 64) - 1));
-    x1.[0] <- (W64.of_int 0);
-    x1.[1] <- (W64.of_int 0);
-    x1.[2] <- (W64.of_int 0);
-    x1.[3] <- (W64.of_int 0);
-    x2.[0] <- (W64.of_int 0);
-    x2.[1] <- (W64.of_int 0);
-    x2.[2] <- (W64.of_int 0);
-    x2.[3] <- (W64.of_int 0);
-    d <@ ith_bit (n, ctr);
-    x3.[0] <- x.[0];
-    x3.[1] <- x.[1];
-    x3.[2] <- x.[2];
-    x3.[3] <- x.[3];
-    x4 <@ addm (m, x, x);
-    p <- d;
-    (x1, x3) <@ swapr (x1, x3, d);
-    (x2, x4) <@ swapr (x2, x4, d);
-    
-    while (((W64.of_int 0) \ult ctr)) {
-      lbit <- ctr;
-      ctr <- (ctr - (W64.of_int 1));
-      t1 <@ ith_bit (n, lbit);
-      t2 <@ ith_bit (n, ctr);
-      p <- d;
-      q <- d;
-      d <- (d `|` t2);
-      par <- (t1 `^` t2);
-      (x1, x2) <@ swapr (x1, x2, par);
-      x1 <@ addm (m, x1, x2);
-      x2 <@ addm (m, x2, x2);
-      q <- (q `|` t2);
-      cbit <- (q `^` p);
-      (x1, x3) <@ swapr (x1, x3, cbit);
-      (x2, x4) <@ swapr (x2, x4, cbit);
+    z <@ dbn_copy (x);
+    (cf, z) <@ dbn_subc (z, p);
+    i <- 0;
+    while (i < 8) {
+      r1 <- z.[i];
+      r2 <- x.[i];
+      r1 <- (cf ? r2 : r1);
+      x.[i] <- r1;
+      i <- i + 1;
     }
-    par <@ ith_bit (n, (W64.of_int 0));
-    (x1, x2) <@ swapr (x2, x1, par);
-    return (x1);
+    return (x);
+  }
+  
+  proc bn_expand (x:W64.t Array4.t) : W64.t Array8.t = {
+    var aux: int;
+    
+    var r:W64.t Array8.t;
+    var i:int;
+    r <- witness;
+    i <- 0;
+    while (i < 4) {
+      r.[i] <- x.[i];
+      i <- i + 1;
+    }
+
+    while (i < 8) {
+      r.[i] <- (W64.of_int 0);
+      i <- i + 1;
+    }
+    return (r);
+  }
+  
+  proc bn_shrink (x:W64.t Array8.t) : W64.t Array4.t = {
+    var aux: int;
+    
+    var r:W64.t Array4.t;
+    var i:int;
+    r <- witness;
+    i <- 0;
+    while (i < 4) {
+      r.[i] <- x.[i];
+      i <- i + 1;
+    }
+    return (r);
+  }
+  
+  proc div2 (x:W64.t Array16.t, k:int) : W64.t Array8.t = {
+    var aux: int;
+    
+    var r:W64.t Array8.t;
+    var i:int;
+    r <- witness;
+    aux <- k;
+    i <- 0;
+    while (i < aux) {
+      r.[i] <- x.[(8 + i)];
+      i <- i + 1;
+    }
+    return (r);
+  }
+  
+  proc bnreduce (a:W64.t Array8.t, r:W64.t Array8.t, p:W64.t Array4.t) : 
+  W64.t Array4.t = {
+    return p;
+    
+    (* var res_0:W64.t Array4.t; *)
+    (* var xr:W64.t Array16.t; *)
+    (* var xrf:W64.t Array8.t; *)
+    (* var xrfn:W64.t Array8.t; *)
+    (* var t:W64.t Array8.t; *)
+    (* var pp:W64.t Array8.t; *)
+    (* var  _0:W64.t; *)
+    (* var  _1:bool; *)
+    (* var  _2:bool; *)
+    (* var  _3:W64.t; *)
+    (* var  _4:bool; *)
+    (* var  _5:bool; *)
+    (* var  _6:bool; *)
+    (* pp <- witness; *)
+    (* res_0 <- witness; *)
+    (* t <- witness; *)
+    (* xr <- witness; *)
+    (* xrf <- witness; *)
+    (* xrfn <- witness; *)
+    (* ( _0,  _1,  _2, xr) <@ dbn_muln (a, r); *)
+    (* xrf <@ div2 (xr, (2 * 4)); *)
+    (* pp <@ bn_expand (p); *)
+    (* ( _3,  _4,  _5, xrfn) <@ dbn_muln (xrf, pp); *)
+    (* ( _6, t) <@ dbn_subc (a, xrfn); *)
+
+    (* t <@ dcminusP (pp, t); *)
+    (* res_0 <@ bn_shrink (t); *)
+    (* return (res_0); *)
   }
   
   proc toEC () : unit = {
     
+    var z:W64.t Array8.t;
     var p:W64.t Array4.t;
-    var a:W64.t Array4.t;
-    var b:W64.t Array4.t;
     var r:W64.t Array4.t;
-    var x:W64.t;
-    var  _0:W64.t Array4.t;
-     _0 <- witness;
-    a <- witness;
-    b <- witness;
     p <- witness;
     r <- witness;
-    r <@ addm (p, a, b);
-    r <@ mulm (p, a, b);
-    x <@ ith_bit (a, x);
-    ( _0, a) <@ swapr (a, a, x);
+    z <- witness;
+    r <@ bnreduce (z, z, p);
     return ();
   }
 }.
