w64x4/proof/Fp_w64x4_extract_ct.ec
@@ -1,15 +1,16 @@
 require import AllCore IntDiv CoreMap List Distr.
-require import JModel.
+from Jasmin require import JModel.
 
-require import Array4.
-require import WArray32.
+require import Array32.
+require import WArray256.
 
 
 
 module M = {
   var leakages : leakages_t
   
-  proc bn_subc (a:W64.t Array4.t, b:W64.t Array4.t) : bool * W64.t Array4.t = {
+  proc bn_subc (a:W64.t Array32.t, b:W64.t Array32.t) : bool *
+                                                        W64.t Array32.t = {
     var aux_0: bool;
     var aux_1: int;
     var aux: W64.t;
@@ -26,16 +27,16 @@ module M = {
     aux <- b.[0];
     x2 <- aux;
     leakages <- LeakAddr([]) :: leakages;
-    (aux_0, aux) <- subc_64 x1 x2 false;
+    (aux_0, aux) <- sbb_64 x1 x2 false;
     cf <- aux_0;
     x1 <- aux;
     leakages <- LeakAddr([]) :: leakages;
     aux <- x1;
     leakages <- LeakAddr([0]) :: leakages;
     a.[0] <- aux;
-    leakages <- LeakFor(1,4) :: LeakAddr([]) :: leakages;
+    leakages <- LeakFor(1,32) :: LeakAddr([]) :: leakages;
     i <- 1;
-    while (i < 4) {
+    while (i < 32) {
       leakages <- LeakAddr([i]) :: leakages;
       aux <- a.[i];
       x1 <- aux;
@@ -43,7 +44,7 @@ module M = {
       aux <- b.[i];
       x2 <- aux;
       leakages <- LeakAddr([]) :: leakages;
-      (aux_0, aux) <- subc_64 x1 x2 cf;
+      (aux_0, aux) <- sbb_64 x1 x2 cf;
       cf <- aux_0;
       x1 <- aux;
       leakages <- LeakAddr([]) :: leakages;
@@ -55,7 +56,49 @@ module M = {
     return (cf, a);
   }
   
-  proc bn_addc (a:W64.t Array4.t, b:W64.t Array4.t) : bool * W64.t Array4.t = {
+  proc bn_copy (a:W64.t Array32.t) : W64.t Array32.t = {
+    var aux: int;
+    var aux_0: W64.t;
+    
+    var r:W64.t Array32.t;
+    var i:int;
+    var t:W64.t;
+    r <- witness;
+    leakages <- LeakFor(0,32) :: LeakAddr([]) :: leakages;
+    i <- 0;
+    while (i < 32) {
+      leakages <- LeakAddr([i]) :: leakages;
+      aux_0 <- a.[i];
+      t <- aux_0;
+      leakages <- LeakAddr([]) :: leakages;
+      aux_0 <- t;
+      leakages <- LeakAddr([i]) :: leakages;
+      r.[i] <- aux_0;
+      i <- i + 1;
+    }
+    return (r);
+  }
+  
+  proc bn_set0 (a:W64.t Array32.t) : W64.t Array32.t = {
+    var aux: int;
+    var aux_0: W64.t;
+    
+    var i:int;
+    
+    leakages <- LeakFor(0,32) :: LeakAddr([]) :: leakages;
+    i <- 0;
+    while (i < 32) {
+      leakages <- LeakAddr([]) :: leakages;
+      aux_0 <- (W64.of_int 0);
+      leakages <- LeakAddr([i]) :: leakages;
+      a.[i] <- aux_0;
+      i <- i + 1;
+    }
+    return (a);
+  }
+  
+  proc bn_addc (a:W64.t Array32.t, b:W64.t Array32.t) : bool *
+                                                        W64.t Array32.t = {
     var aux_0: bool;
     var aux_1: int;
     var aux: W64.t;
@@ -72,16 +115,16 @@ module M = {
     aux <- b.[0];
     x2 <- aux;
     leakages <- LeakAddr([]) :: leakages;
-    (aux_0, aux) <- addc_64 x1 x2 false;
+    (aux_0, aux) <- adc_64 x1 x2 false;
     cf <- aux_0;
     x1 <- aux;
     leakages <- LeakAddr([]) :: leakages;
     aux <- x1;
     leakages <- LeakAddr([0]) :: leakages;
     a.[0] <- aux;
-    leakages <- LeakFor(1,4) :: LeakAddr([]) :: leakages;
+    leakages <- LeakFor(1,32) :: LeakAddr([]) :: leakages;
     i <- 1;
-    while (i < 4) {
+    while (i < 32) {
       leakages <- LeakAddr([i]) :: leakages;
       aux <- a.[i];
       x1 <- aux;
@@ -89,7 +132,7 @@ module M = {
       aux <- b.[i];
       x2 <- aux;
       leakages <- LeakAddr([]) :: leakages;
-      (aux_0, aux) <- addc_64 x1 x2 cf;
+      (aux_0, aux) <- adc_64 x1 x2 cf;
       cf <- aux_0;
       x1 <- aux;
       leakages <- LeakAddr([]) :: leakages;
@@ -99,6 +142,50 @@ module M = {
       i <- i + 1;
     }
     return (cf, a);
+  }
+  
+  proc swapr (x:W64.t Array32.t, y:W64.t Array32.t, swap_0:W64.t) : W64.t Array32.t *
+                                                                    W64.t Array32.t = {
+    var aux_0: int;
+    var aux: W64.t;
+    
+    var mask:W64.t;
+    var i:int;
+    var tmp1:W64.t;
+    var tmp2:W64.t;
+    
+    leakages <- LeakAddr([]) :: leakages;
+    aux <- (swap_0 * (W64.of_int 18446744073709551615));
+    mask <- aux;
+    leakages <- LeakFor(0,32) :: LeakAddr([]) :: leakages;
+    i <- 0;
+    while (i < 32) {
+      leakages <- LeakAddr([i]) :: leakages;
+      aux <- x.[i];
+      tmp1 <- aux;
+      leakages <- LeakAddr([i]) :: leakages;
+      aux <- (tmp1 `^` y.[i]);
+      tmp1 <- aux;
+      leakages <- LeakAddr([]) :: leakages;
+      aux <- (tmp1 `&` mask);
+      tmp1 <- aux;
+      leakages <- LeakAddr([i]) :: leakages;
+      aux <- (x.[i] `^` tmp1);
+      leakages <- LeakAddr([i]) :: leakages;
+      x.[i] <- aux;
+      leakages <- LeakAddr([i]) :: leakages;
+      aux <- y.[i];
+      tmp2 <- aux;
+      leakages <- LeakAddr([]) :: leakages;
+      aux <- (tmp2 `^` tmp1);
+      tmp2 <- aux;
+      leakages <- LeakAddr([]) :: leakages;
+      aux <- tmp2;
+      leakages <- LeakAddr([i]) :: leakages;
+      y.[i] <- aux;
+      i <- i + 1;
+    }
+    return (x, y);
   }
   
   proc ith_bit64 (k:W64.t, ctr:W64.t) : W64.t = {
@@ -125,7 +212,7 @@ module M = {
     return (bit);
   }
   
-  proc ith_bit (kk:W64.t Array4.t, ctr:W64.t) : W64.t = {
+  proc ith_bit (kk:W64.t Array32.t, ctr:W64.t) : W64.t = {
     var aux: W64.t;
     
     var bit:W64.t;
@@ -156,251 +243,100 @@ module M = {
     return (bit);
   }
   
-  proc swapr (x:W64.t Array4.t, y:W64.t Array4.t, swap_0:W64.t) : W64.t Array4.t *
-                                                                  W64.t Array4.t = {
-    var aux_0: int;
-    var aux: W64.t;
-    
-    var mask:W64.t;
-    var i:int;
-    var tmp1:W64.t;
-    var tmp2:W64.t;
-    
-    leakages <- LeakAddr([]) :: leakages;
-    aux <- (swap_0 * (W64.of_int 18446744073709551615));
-    mask <- aux;
-    leakages <- LeakFor(0,4) :: LeakAddr([]) :: leakages;
-    i <- 0;
-    while (i < 4) {
-      leakages <- LeakAddr([i]) :: leakages;
-      aux <- x.[i];
-      tmp1 <- aux;
-      leakages <- LeakAddr([i]) :: leakages;
-      aux <- (tmp1 `^` y.[i]);
-      tmp1 <- aux;
-      leakages <- LeakAddr([]) :: leakages;
-      aux <- (tmp1 `&` mask);
-      tmp1 <- aux;
-      leakages <- LeakAddr([i]) :: leakages;
-      aux <- (x.[i] `^` tmp1);
-      leakages <- LeakAddr([i]) :: leakages;
-      x.[i] <- aux;
-      leakages <- LeakAddr([i]) :: leakages;
-      aux <- y.[i];
-      tmp2 <- aux;
-      leakages <- LeakAddr([]) :: leakages;
-      aux <- (tmp2 `^` tmp1);
-      tmp2 <- aux;
-      leakages <- LeakAddr([]) :: leakages;
-      aux <- tmp2;
-      leakages <- LeakAddr([i]) :: leakages;
-      y.[i] <- aux;
-      i <- i + 1;
-    }
-    return (x, y);
-  }
-  
-  proc cminusP (p:W64.t Array4.t, x:W64.t Array4.t) : W64.t Array4.t = {
+  proc cminusP (p:W64.t Array32.t, x:W64.t Array32.t) : W64.t Array32.t = {
     var aux_0: bool;
-    var aux: W64.t;
-    var aux_1: W64.t Array4.t;
+    var aux_1: int;
+    var aux_2: W64.t;
+    var aux: W64.t Array32.t;
     
-    var t:W64.t Array4.t;
-    var z:W64.t Array4.t;
+    var z:W64.t Array32.t;
     var cf:bool;
+    var i:int;
     var r1:W64.t;
     var r2:W64.t;
-    t <- witness;
     z <- witness;
-    leakages <- LeakAddr([0]) :: leakages;
-    aux <- x.[0];
-    leakages <- LeakAddr([0]) :: leakages;
-    z.[0] <- aux;
-    leakages <- LeakAddr([1]) :: leakages;
-    aux <- x.[1];
-    leakages <- LeakAddr([1]) :: leakages;
-    z.[1] <- aux;
-    leakages <- LeakAddr([2]) :: leakages;
-    aux <- x.[2];
-    leakages <- LeakAddr([2]) :: leakages;
-    z.[2] <- aux;
-    leakages <- LeakAddr([3]) :: leakages;
-    aux <- x.[3];
-    leakages <- LeakAddr([3]) :: leakages;
-    z.[3] <- aux;
     leakages <- LeakAddr([]) :: leakages;
-    (aux_0, aux_1) <@ bn_subc (z, p);
+    aux <@ bn_copy (x);
+    z <- aux;
+    leakages <- LeakAddr([]) :: leakages;
+    (aux_0, aux) <@ bn_subc (z, p);
     cf <- aux_0;
-    t <- aux_1;
-    leakages <- LeakAddr([0]) :: leakages;
-    aux <- t.[0];
-    r1 <- aux;
-    leakages <- LeakAddr([0]) :: leakages;
-    aux <- x.[0];
-    r2 <- aux;
-    leakages <- LeakAddr([]) :: leakages;
-    aux <- (cf ? r2 : r1);
-    r1 <- aux;
-    leakages <- LeakAddr([]) :: leakages;
-    aux <- r1;
-    leakages <- LeakAddr([0]) :: leakages;
-    t.[0] <- aux;
-    leakages <- LeakAddr([1]) :: leakages;
-    aux <- t.[1];
-    r1 <- aux;
-    leakages <- LeakAddr([1]) :: leakages;
-    aux <- x.[1];
-    r2 <- aux;
-    leakages <- LeakAddr([]) :: leakages;
-    aux <- (cf ? r2 : r1);
-    r1 <- aux;
-    leakages <- LeakAddr([]) :: leakages;
-    aux <- r1;
-    leakages <- LeakAddr([1]) :: leakages;
-    t.[1] <- aux;
-    leakages <- LeakAddr([2]) :: leakages;
-    aux <- t.[2];
-    r1 <- aux;
-    leakages <- LeakAddr([2]) :: leakages;
-    aux <- x.[2];
-    r2 <- aux;
-    leakages <- LeakAddr([]) :: leakages;
-    aux <- (cf ? r2 : r1);
-    r1 <- aux;
-    leakages <- LeakAddr([]) :: leakages;
-    aux <- r1;
-    leakages <- LeakAddr([2]) :: leakages;
-    t.[2] <- aux;
-    leakages <- LeakAddr([3]) :: leakages;
-    aux <- t.[3];
-    r1 <- aux;
-    leakages <- LeakAddr([3]) :: leakages;
-    aux <- x.[3];
-    r2 <- aux;
-    leakages <- LeakAddr([]) :: leakages;
-    aux <- (cf ? r2 : r1);
-    r1 <- aux;
-    leakages <- LeakAddr([]) :: leakages;
-    aux <- r1;
-    leakages <- LeakAddr([3]) :: leakages;
-    t.[3] <- aux;
-    return (t);
+    z <- aux;
+    leakages <- LeakFor(0,32) :: LeakAddr([]) :: leakages;
+    i <- 0;
+    while (i < 32) {
+      leakages <- LeakAddr([i]) :: leakages;
+      aux_2 <- z.[i];
+      r1 <- aux_2;
+      leakages <- LeakAddr([i]) :: leakages;
+      aux_2 <- x.[i];
+      r2 <- aux_2;
+      leakages <- LeakAddr([]) :: leakages;
+      aux_2 <- (cf ? r2 : r1);
+      r1 <- aux_2;
+      leakages <- LeakAddr([]) :: leakages;
+      aux_2 <- r1;
+      leakages <- LeakAddr([i]) :: leakages;
+      x.[i] <- aux_2;
+      i <- i + 1;
+    }
+    return (x);
   }
   
-  proc addm (p:W64.t Array4.t, a:W64.t Array4.t, b:W64.t Array4.t) : 
-  W64.t Array4.t = {
+  proc addm (p:W64.t Array32.t, a:W64.t Array32.t, b:W64.t Array32.t) : 
+  W64.t Array32.t = {
     var aux: bool;
-    var aux_1: W64.t;
-    var aux_0: W64.t Array4.t;
+    var aux_0: W64.t Array32.t;
     
-    var f:W64.t Array4.t;
-    var z:W64.t Array4.t;
     var  _0:bool;
-    f <- witness;
-    z <- witness;
+    
     leakages <- LeakAddr([]) :: leakages;
     (aux, aux_0) <@ bn_addc (a, b);
      _0 <- aux;
-    f <- aux_0;
-    leakages <- LeakAddr([0]) :: leakages;
-    aux_1 <- f.[0];
-    leakages <- LeakAddr([0]) :: leakages;
-    z.[0] <- aux_1;
-    leakages <- LeakAddr([1]) :: leakages;
-    aux_1 <- f.[1];
-    leakages <- LeakAddr([1]) :: leakages;
-    z.[1] <- aux_1;
-    leakages <- LeakAddr([2]) :: leakages;
-    aux_1 <- f.[2];
-    leakages <- LeakAddr([2]) :: leakages;
-    z.[2] <- aux_1;
-    leakages <- LeakAddr([3]) :: leakages;
-    aux_1 <- f.[3];
-    leakages <- LeakAddr([3]) :: leakages;
-    z.[3] <- aux_1;
+    a <- aux_0;
     leakages <- LeakAddr([]) :: leakages;
-    aux_0 <@ cminusP (p, z);
-    f <- aux_0;
-    return (f);
+    aux_0 <@ cminusP (p, a);
+    a <- aux_0;
+    return (a);
   }
   
-  proc mulm (m:W64.t Array4.t, x:W64.t Array4.t, n:W64.t Array4.t) : 
-  W64.t Array4.t = {
+  proc mulm (m:W64.t Array32.t, x:W64.t Array32.t, n:W64.t Array32.t) : 
+  W64.t Array32.t = {
     var aux: W64.t;
-    var aux_1: W64.t Array4.t;
-    var aux_0: W64.t Array4.t;
+    var aux_1: W64.t Array32.t;
+    var aux_0: W64.t Array32.t;
     
-    var x1:W64.t Array4.t;
+    var x1:W64.t Array32.t;
     var ctr:W64.t;
-    var x2:W64.t Array4.t;
+    var x2:W64.t Array32.t;
     var d:W64.t;
-    var x3:W64.t Array4.t;
-    var x4:W64.t Array4.t;
+    var x3:W64.t Array32.t;
+    var x4:W64.t Array32.t;
     var p:W64.t;
     var lbit:W64.t;
     var t1:W64.t;
     var t2:W64.t;
     var q:W64.t;
     var par:W64.t;
-    var cbit:W64.t;
     x1 <- witness;
     x2 <- witness;
     x3 <- witness;
     x4 <- witness;
     leakages <- LeakAddr([]) :: leakages;
-    aux <- (W64.of_int ((4 * 64) - 1));
+    aux <- (W64.of_int ((32 * 64) - 1));
     ctr <- aux;
     leakages <- LeakAddr([]) :: leakages;
-    aux <- (W64.of_int 0);
-    leakages <- LeakAddr([0]) :: leakages;
-    x1.[0] <- aux;
+    aux_1 <@ bn_set0 (x1);
+    x1 <- aux_1;
     leakages <- LeakAddr([]) :: leakages;
-    aux <- (W64.of_int 0);
-    leakages <- LeakAddr([1]) :: leakages;
-    x1.[1] <- aux;
-    leakages <- LeakAddr([]) :: leakages;
-    aux <- (W64.of_int 0);
-    leakages <- LeakAddr([2]) :: leakages;
-    x1.[2] <- aux;
-    leakages <- LeakAddr([]) :: leakages;
-    aux <- (W64.of_int 0);
-    leakages <- LeakAddr([3]) :: leakages;
-    x1.[3] <- aux;
-    leakages <- LeakAddr([]) :: leakages;
-    aux <- (W64.of_int 0);
-    leakages <- LeakAddr([0]) :: leakages;
-    x2.[0] <- aux;
-    leakages <- LeakAddr([]) :: leakages;
-    aux <- (W64.of_int 0);
-    leakages <- LeakAddr([1]) :: leakages;
-    x2.[1] <- aux;
-    leakages <- LeakAddr([]) :: leakages;
-    aux <- (W64.of_int 0);
-    leakages <- LeakAddr([2]) :: leakages;
-    x2.[2] <- aux;
-    leakages <- LeakAddr([]) :: leakages;
-    aux <- (W64.of_int 0);
-    leakages <- LeakAddr([3]) :: leakages;
-    x2.[3] <- aux;
+    aux_1 <@ bn_set0 (x2);
+    x2 <- aux_1;
     leakages <- LeakAddr([]) :: leakages;
     aux <@ ith_bit (n, ctr);
     d <- aux;
-    leakages <- LeakAddr([0]) :: leakages;
-    aux <- x.[0];
-    leakages <- LeakAddr([0]) :: leakages;
-    x3.[0] <- aux;
-    leakages <- LeakAddr([1]) :: leakages;
-    aux <- x.[1];
-    leakages <- LeakAddr([1]) :: leakages;
-    x3.[1] <- aux;
-    leakages <- LeakAddr([2]) :: leakages;
-    aux <- x.[2];
-    leakages <- LeakAddr([2]) :: leakages;
-    x3.[2] <- aux;
-    leakages <- LeakAddr([3]) :: leakages;
-    aux <- x.[3];
-    leakages <- LeakAddr([3]) :: leakages;
-    x3.[3] <- aux;
+    leakages <- LeakAddr([]) :: leakages;
+    aux_1 <@ bn_copy (x);
+    x3 <- aux_1;
     leakages <- LeakAddr([]) :: leakages;
     aux_1 <@ addm (m, x, x);
     x4 <- aux_1;
@@ -450,23 +386,6 @@ module M = {
       leakages <- LeakAddr([]) :: leakages;
       aux_1 <@ addm (m, x1, x2);
       x1 <- aux_1;
-      leakages <- LeakAddr([]) :: leakages;
-      aux_1 <@ addm (m, x2, x2);
-      x2 <- aux_1;
-      leakages <- LeakAddr([]) :: leakages;
-      aux <- (q `|` t2);
-      q <- aux;
-      leakages <- LeakAddr([]) :: leakages;
-      aux <- (q `^` p);
-      cbit <- aux;
-      leakages <- LeakAddr([]) :: leakages;
-      (aux_1, aux_0) <@ swapr (x1, x3, cbit);
-      x1 <- aux_1;
-      x3 <- aux_0;
-      leakages <- LeakAddr([]) :: leakages;
-      (aux_1, aux_0) <@ swapr (x2, x4, cbit);
-      x2 <- aux_1;
-      x4 <- aux_0;
     leakages <- LeakCond(((W64.of_int 0) \ult ctr)) :: LeakAddr([]) :: leakages;
     
     }
@@ -481,19 +400,34 @@ module M = {
   }
   
   proc toEC () : unit = {
-    var aux: W64.t Array4.t;
+    var aux_0: W64.t;
+    var aux_1: W64.t Array32.t;
+    var aux: W64.t Array32.t;
     
-    var p:W64.t Array4.t;
-    var a:W64.t Array4.t;
-    var b:W64.t Array4.t;
-    var r:W64.t Array4.t;
+    var p:W64.t Array32.t;
+    var a:W64.t Array32.t;
+    var b:W64.t Array32.t;
+    var r:W64.t Array32.t;
+    var x:W64.t;
+    var  _0:W64.t Array32.t;
+     _0 <- witness;
     a <- witness;
     b <- witness;
     p <- witness;
     r <- witness;
     leakages <- LeakAddr([]) :: leakages;
-    aux <@ mulm (p, a, b);
-    r <- aux;
+    aux_1 <@ addm (p, a, b);
+    r <- aux_1;
+    leakages <- LeakAddr([]) :: leakages;
+    aux_1 <@ mulm (p, a, b);
+    r <- aux_1;
+    leakages <- LeakAddr([]) :: leakages;
+    aux_0 <@ ith_bit (a, x);
+    x <- aux_0;
+    leakages <- LeakAddr([]) :: leakages;
+    (aux_1, aux) <@ swapr (a, a, x);
+     _0 <- aux_1;
+    a <- aux;
     return ();
   }
 }.
