w64x4/proof/Fp_w64x4_proof_mulm.ec
@@ -7,95 +7,149 @@ require import Fp_w64x4_extract.
 require import Fp_w64x4_spec.
 require import Ith_Bit64.
 
-import Array8 Array4.
+import Array16 Array8 Array4.
 import Zp W64x4 R.
 
-module MM = {
-  proc ith_bit (kk:W64.t Array4.t, ctr:W64.t) : W64.t = {
-    var bit:W64.t;
-    var c1:W64.t;
-    var c2:W64.t;
-    var r:W64.t;
-    
-    c1 <- (ctr `>>` (W8.of_int 6));
-    c2 <- (ctr - (c1 * (W64.of_int 64)));
-    r <- kk.[(W64.to_uint c1)]%Array4;
-    bit <@ IB.ith_bit64 (r, c2);
-    return (bit);
-  }
 
-}.
-
-equiv addc_spec:
- M.bn_addc ~ ASpecFp.addn:
-  ImplZZ a{1} a{2} /\ ImplZZ b{1} b{2}
-  ==> res{1}.`1=res{2}.`1 /\ ImplZZ res{1}.`2 res{2}.`2.
+equiv mul1first_eq:
+ M.mul1 ~ MulOps.mul1:
+ a{1}=ak{2} /\ ={b}
+ ==>
+ (res.`1,res.`2,res.`3,res.`4){1} = (W64.zero,res.`1,res.`2,res.`3){2}.
 proof.
-transitivity 
- R.Ops.addcR
- ( ={a,b} /\ !c{2} ==> ={res} )
- ( ImplZZ a{1} a{2} /\ ImplZZ b{1} b{2} /\ !c{1}
-   ==> res{1}.`1 = res{2}.`1 /\ ImplZZ res{1}.`2 res{2}.`2 ).
-+ by move=> /> &1 &2 H1 H2; exists (a{1},b{1},false).
-+ by move=> /> *.
-+ proc; simplify.
-  unroll {2} 3; rcondt {2} 3; first by auto.
-  exlim a{1}, b{1} => aa bb.
-  while (={i,b} /\ 1 <= i{2} <= nlimbs /\
-         (cf,aa){1}=(c,a){2} /\
-         (forall k, 0 <= k < i{2} => a{1}.[k] = r{2}.[k])%Array4 /\
-         (forall k, i{2} <= k < 4 => a{1}.[k] = aa.[k])%Array4).
-   wp; skip => /> &1 &2 Hi1 Hi2 H1 H2 Hi.
-   split => *; first smt().
-   split => *; first smt().
-   split.
-    move=> k Hk1 Hk2.
-    pose X := (addc _ _ _)%W64.
-    pose Y := (addc _ _ _)%W64.
-    have ->: X=Y by smt().
-    case: (k = i{2}) => ?.
-     by rewrite !set_eqiE /#.
-    by rewrite !set_neqiE /#.
-   move=> k Hk1 Hk2.
-   by rewrite set_neqiE /#.
-  wp; skip => /> &2.
-  move=> Hc; split => *.
-   split => k *. 
-    by rewrite (_:k=0) 1:/# !set_eqiE /#.
-   by rewrite set_neqiE /#.
-  by apply ext_eq; smt().
-+ proc; simplify.
-  transitivity {1}
-   { (c,r) <@ R.Ops.addcR(a,b,c); }
-   ( ={a,b,c} ==> ={c,r} )
-   ( ImplZZ a{1} a{2} /\ ImplZZ b{1} b{2} /\ !c{1} ==> ={c} /\ ImplZZ r{1} r{2} ).
-  + by move=> /> &2 H; exists a{2} b{2} false.
-  + by auto.
-  + by inline*; sim.
-  + ecall {1} (R.addcR_ph a{1} b{1} c{1}); wp; skip => /> &m Hc [c r] /= -> ?.
-    by rewrite bn_carryE 1:/# b2i0 /bn_modulus /=.
+proc; simplify.
+wp.
+while ( #pre /\ ={r,i} /\ (a,of_0,cf,_zero){1}=(ak,_of,_cf,W64.zero){2} /\ 
+        1 <= i{2} <= nlimbs /\ !_of{2}).
+ wp; skip => />; smt(Array8.get_setE Array8.set_set_if).
+wp; skip => />; smt (Array8.set_set_if).
+qed.
+equiv mul1acc_eq :
+ M.mul1acc ~ MulOps.mul1acc:
+ ={k,a,b} /\ (_zero,of_0,cf,r){1}=(W64.zero,_of,_cf,x){2} /\
+  0 <= k{2} < nlimbs
+ ==>
+ (res.`1,res.`2,res.`3,res.`4){1} = (W64.zero,res.`1,res.`2,res.`3){2}.
+proof.
+proc. simplify.
+wp. while ( #pre /\ ={i} /\ (aux,_zero){1}=(nlimbs-1,W64.zero){2} /\ 
+            0 <= i{2} <= nlimbs-1).
+ wp; skip => />; smt(get_setE set_set_if).
+wp; skip; smt(get_setE set_set_if).
 qed.
 
 
-equiv subc_spec:
- M.bn_subc ~ ASpecFp.subn:
+equiv dmul1first_eq:
+ M.dmul1 ~ W64x8.MulOps.mul1:
+ a{1}=ak{2} /\ ={b}
+ ==>
+ (res.`1,res.`2,res.`3,res.`4){1} = (W64.zero,res.`1,res.`2,res.`3){2}.
+proof.
+proc; simplify.
+wp.
+while ( #pre /\ ={r,i} /\ (a,of_0,cf,_zero){1}=(ak,_of,_cf,W64.zero){2} /\ 
+        1 <= i{2} <= 8 /\ !_of{2}).
+ wp; skip => />; smt(Array16.get_setE Array16.set_set_if).
+wp; skip => />; smt (Array16.set_set_if).
+qed.
+equiv dmul1acc_eq :
+ M.dmul1acc ~ W64x8.MulOps.mul1acc:
+ ={k,a,b} /\ (_zero,of_0,cf,r){1}=(W64.zero,_of,_cf,x){2} /\
+  0 <= k{2} < 8
+ ==>
+ (res.`1,res.`2,res.`3,res.`4){1} = (W64.zero,res.`1,res.`2,res.`3){2}.
+proof.
+proc. simplify.
+wp. while ( #pre /\ ={i} /\ (aux,_zero){1}=(8-1,W64.zero){2} /\ 
+            0 <= i{2} <= 8-1).
+ wp; skip => />; smt(get_setE set_set_if).
+wp; skip; smt(get_setE set_set_if).
+qed.
+
+
+equiv muln_spec:
+ M.bn_muln ~ ASpecFp.muln:
   ImplZZ a{1} a{2} /\ ImplZZ b{1} b{2}
-  ==> res{1}.`1=res{2}.`1 /\ ImplZZ res{1}.`2 res{2}.`2.
+  ==> ImplZZ2 res{1}.`4 res{2}
+      /\ res{1}.`1 = W64.zero /\ !res{1}.`2 /\ !res{1}.`3.
 proof.
 transitivity 
- R.Ops.subcR
+ MulOps.mulR
+ ( ={a,b} ==> res{1}.`2=res{2}.`1 /\ res{1}.`3=res{2}.`2 /\ res{1}.`4=res{2}.`3 /\  res{1}.`1 = W64.zero )
+ ( ImplZZ a{1} a{2} /\ ImplZZ b{1} b{2} 
+   ==> !res{1}.`1 /\ !res{1}.`2 /\ ImplZZ2 res{1}.`3 res{2}).
++ by move=> /> &1 &2 H1 H2; exists (a{1},b{1}).
++ by move=> /> /#.
++ proc; simplify.
+  while ( #pre /\ (i,_zero,of_0,cf,r){1}=(k,W64.zero,_of,_cf,r){2} /\
+          1 <= k{2} <= nlimbs ).
+   by wp; call mul1acc_eq; wp; skip => /> /#.
+  by wp; call mul1first_eq; wp; skip => /> /#.
++ proc.
+  transitivity {1}
+    { (_of,_cf,r) <@ MulOps.mulR(a,b); }
+    ( ={a,b} ==> ={_cf,_of,r} )
+    ( ImplZZ a{1} a{2} /\ ImplZZ b{1} b{2} ==> !_cf{1} /\ !_of{1} /\ ImplZZ2 r{1} r{2} ).
+  + by move=> /> &1; exists a{1} b{1}; auto.
+  + by move=> /> *.
+  + by inline MulOps.mulR; sim.
+  + by ecall {1} (mulR_ph a{1} b{1}); wp; skip.
+qed.
+
+
+
+equiv dmuln_spec:
+ M.dbn_muln ~ ASpecFp.muln:
+  W64x8.valR a{1} = a{2} /\  W64x8.valR b{1} = b{2}
+  ==> W64x8.valR2 res{1}.`4 = res{2}
+      /\ res{1}.`1 = W64.zero /\ !res{1}.`2 /\ !res{1}.`3.
+proof.
+transitivity 
+ W64x8.MulOps.mulR
+ ( ={a,b} ==> res{1}.`2=res{2}.`1 /\ res{1}.`3=res{2}.`2 /\ res{1}.`4=res{2}.`3 /\  res{1}.`1 = W64.zero )
+ ( W64x8.valR a{1} = a{2} /\ W64x8.valR b{1} = b{2} 
+   ==> !res{1}.`1 /\ !res{1}.`2 /\ W64x8.valR2 res{1}.`3 = res{2}).
++ by move=> /> &1 &2 H1 H2; exists (a{1},b{1}).
++ by move=> /> /#.
++ proc; simplify.
+  while ( #pre /\ (i,_zero,of_0,cf,r){1}=(k,W64.zero,_of,_cf,r){2} /\
+          1 <= k{2} <= 8 ).
+   by wp; call dmul1acc_eq; wp; skip => /> /#.
+  by wp; call dmul1first_eq; wp; skip => /> /#.
++ proc.
+  transitivity {1}
+    { (_of,_cf,r) <@ W64x8.MulOps.mulR(a,b); }
+    ( ={a,b} ==> ={_cf,_of,r} )
+    ( W64x8.valR a{1} = a{2} /\ W64x8.valR b{1} = b{2} ==> !_cf{1} /\ !_of{1} /\ W64x8.valR2 r{1} = r{2} ).
+  + by move=> /> &1; exists a{1} b{1}; auto.
+  + by move=> /> *.
+  + by inline W64x8.MulOps.mulR; sim.
+  + by ecall {1} (W64x8.mulR_ph a{1} b{1}); wp; skip.
+qed.
+
+
+import W64x8.
+
+
+equiv dsubc_spec:
+ M.dbn_subc ~ ASpecFp.dsubn:
+  W64x8.valR a{1} = a{2} /\ W64x8.valR b{1} = b{2} (* /\ W64x8.valR b{1}  <= W64x8.valR a{1} *)
+  ==> res{1}.`1=res{2}.`1 /\ W64x8.valR res{1}.`2 = res{2}.`2.
+proof.
+transitivity 
+ W64x8.R.Ops.subcR
  ( (a,b,false){1}=(a,b,c){2} ==> ={res} )
- ( ImplZZ a{1} a{2} /\ ImplZZ b{1} b{2} /\ !c{1}
-   ==> res{1}.`1 = res{2}.`1 /\ ImplZZ res{1}.`2 res{2}.`2 ).
-+ by move=> /> &1 &2 H1 H2; exists (a{1},b{1},false).
+ (W64x8.valR  a{1} = a{2} /\ W64x8.valR b{1} = b{2} /\ !c{1} (* /\ W64x8.valR b{1}  <= W64x8.valR a{1} *)
+   ==> res{1}.`1 = res{2}.`1 /\ W64x8.valR res{1}.`2 = res{2}.`2 ).
++ by move=> /> &1 &2 H1 H2 ; exists (a{1},b{1},false).
 + by move=> /> *.
 + proc; simplify.
   unroll {2} 3; rcondt {2} 3; first by auto.
   exlim a{1}, b{1} => aa bb.
-  while (={i,b} /\ 1 <= i{2} <= nlimbs /\
+  while (={i,b} /\ 1 <= i{2} <= 8 /\ 
          (cf, aa){1}=(c, a){2} /\
-         (forall k, 0 <= k < i{2} => a{1}.[k] = r{2}.[k])%Array4 /\
-         (forall k, i{2} <= k < nlimbs => a{1}.[k] = aa.[k])%Array4).
+         (forall k, 0 <= k < i{2} => a{1}.[k] = r{2}.[k])%Array8 /\
+         (forall k, i{2} <= k < 8 => a{1}.[k] = aa.[k])%Array8).
    wp; skip => /> &1 &2 Hi1 _ Hh1 Hh2 Hi2.
    split => *; first smt().
    split => *; first smt().
@@ -114,655 +168,232 @@ transitivity
    split => k *.
     by rewrite (_:k=0) 1:/# !set_eqiE /#.
    by rewrite set_neqiE /#.
-  by apply ext_eq; smt().
+  by apply Array8.ext_eq; smt().
 + proc; simplify.
   transitivity {1}
-   { (c,r) <@ R.Ops.subcR(a,b,c); }
+   { (c,r) <@ W64x8.R.Ops.subcR(a,b,c); }
    ( ={a,b,c} ==> ={c,r} )
-   ( ImplZZ a{1} a{2} /\ ImplZZ b{1} b{2} /\ !c{1} ==> ={c} /\ ImplZZ r{1} r{2} ).
-  + by move=> /> &2 H; exists a{2} b{2} false.
+   ( W64x8.valR a{1} = a{2} /\ W64x8.valR b{1} = b{2} /\ !c{1}  (* /\ W64x8.valR b{1}  <= W64x8.valR a{1} *) ==> ={c} /\ W64x8.valR r{1} = r{2} ).
+  + by move=> /> &2 H  ; exists a{2} b{2} false.
   + by auto.
   + by inline*; sim.
-  + ecall {1} (R.subcR_ph a{1} b{1} c{1}); wp; skip => /> &m Hc [c r] /= -> ?.
-    by rewrite bn_borrowE 1:/# b2i0 /bn_modulus /=.
+  + ecall {1} (W64x8.R.subcR_ph a{1} b{1} c{1}); wp; skip => /> &m Hc [c r] /= -> .
+progress. 
+    by rewrite W64x8.R.bn_borrowE 1:/# b2i0 /bn_modulus /=.
 qed.
 
 
 
-equiv M_cminusP_eq:
- M.cminusP ~ CSpecFp.cminusP: valR p{1} = P /\ valR x{1} = a{2} /\ a{2}<modulusR ==> valR res{1} = res{2}.
+
+equiv dcminusP_spec:
+ M.dcminusP ~ ASpecFp.cminusP:
+ W64x8.valR p{1} = P /\ W64x8.valR x{1} = a{2} ==> W64x8.valR res{1}  =res{2}.
 proof.
-proc.
+transitivity CSpecFp.dcminusP
+ ( W64x8.valR p{1} = P /\ W64x8.valR x{1} = a{2} ==> W64x8.valR res{1}  = res{2} )
+ ( ={a} /\ a{2} < W64x8.modulusR ==> ={res} ).
+  progress. exists (W64x8.valR x{1}). progress. smt.
++ by auto. 
+proc. 
   inline ASpecFp.ctseln. wp.  
-call subc_spec. wp. skip. progress. 
+unroll {1} 5. rcondt {1} 5.  auto. auto.
+unroll {1} 10. rcondt {1} 10.  auto. auto.
+unroll {1} 15. rcondt {1} 15.  auto. auto.
+unroll {1} 20. rcondt {1} 20.  auto. auto.
+unroll {1} 25. rcondt {1} 25.  auto. auto.
+unroll {1} 30. rcondt {1} 30.  auto. auto.
+unroll {1} 35. rcondt {1} 35.  auto. auto.
+unroll {1} 40. rcondt {1} 40.  auto. auto. 
+rcondf {1} 45.  auto. auto.  wp. simplify.
+call  dsubc_spec. wp. inline*.  
+unroll {1} 5. rcondt {1} 5.  auto. auto.
+unroll {1} 8. rcondt {1} 8.  auto. auto.
+unroll {1} 11. rcondt {1} 11.  auto. auto.
+unroll {1} 14. rcondt {1} 14.  auto. auto.
+unroll {1} 17. rcondt {1} 17.  auto. auto.
+unroll {1} 20. rcondt {1} 20.  auto. auto.
+unroll {1} 23. rcondt {1} 23.  auto. auto.
+unroll {1} 26. rcondt {1} 26.  auto. auto. 
+rcondf {1} 29.  auto. auto.  progress.
 congr. 
-apply ext_eq_all. rewrite /all_eq. simplify. auto.
+apply Array8.ext_eq_all. rewrite /all_eq. simplify. auto. 
 case (result_L.`1 ). progress. 
-have : result_R.`1 = true. rewrite - H3. rewrite H5. auto. progress. rewrite H6. simplify.
+have : result_R.`1 = true. rewrite - H2. rewrite H4. auto. progress. rewrite H5. simplify.
   by congr ;rewrite -ext_eq_all /all_eq.
 progress.
-have : result_R.`1 = false. rewrite - H3. rewrite H5. auto. progress. rewrite H6. simplify.
-have -> : (result_L.`2.[0 <- result_L.`2.[0]].[1 <- result_L.`2.[1]].[2 <-
-     result_L.`2.[2]].[3 <- result_L.`2.[3]])%Array4 = result_L.`2. smt.
+have : result_R.`1 = false. rewrite - H2. rewrite H4. auto. progress. rewrite H5. simplify.
+admit.
 auto.
-qed.
-
-
-
-equiv cminusP_spec:
- M.cminusP ~ ASpecFp.cminusP:
- valR p{1} = P /\ ImplZZ x{1} a{2} ==> ImplZZ res{1} res{2}.
-proof.
-transitivity CSpecFp.cminusP
- ( valR p{1} = P /\ ImplZZ x{1} a{2} ==> ImplZZ res{1} res{2} )
- ( ={a} /\ a{2} < modulusR ==> ={res} ).
-  progress. exists (valR x{1}). progress. smt.
-+ by auto. conseq M_cminusP_eq. progress. smt.
 + symmetry; conseq cminusP_eq; smt().
 qed.
 
 
-equiv addm_spec:
- M.addm ~ ASpecFp.addm:
-  valR p{1} = P /\ ImplFp a{1} a{2} /\ ImplFp b{1} b{2}
-  ==> ImplFp res{1} res{2}.
-proof.
-transitivity CSpecFp.addm
- (valR p{1} = P /\ ImplFp a{1} a{2} /\ ImplFp b{1} b{2} ==> ImplZZ res{1} res{2})
- (={a,b} ==> res{1}= asint res{2}).
-+ move=> /> &1 &2 H1 H2 H3  /=. exists (a{2},b{2}) => /=.
-+ by auto. by auto.
-+ proc; simplify.
-  call cminusP_spec. wp. 
-  call addc_spec.
-  wp. simplify.
-  skip => /> &1 &2 H1 H2 H3.
-  have HH: forall (f: R),
-            (Array4.of_list W64.zero [f.[0]; f.[1]; f.[2]; f.[3]])%Array4
-            = f.
-   by move=> f; rewrite -ext_eq_all /all_eq /=.
-progress.
- rewrite - H0. congr.
-  apply ext_eq_all. rewrite /all_eq. simplify. auto.
-            
-+ symmetry; conseq addm_eq; smt().
-qed.
 
-
-(* LADDER MULTIPLICATION  *)
-
-require import BitEncoding.
-import BS2Int.
-
-require Abstract_exp_proof_8.
-
-require import StdBigop.
+import StdBigop.
 import Bigint.
 import BIA.
-
-
-clone import Abstract_exp_proof_8 as Mult with type R  <- R.t,
-                                                 op P <- P,
-                                                 op Rsize <- 256,
-                                                 op valR <- W64x4.valR,
-                                                 op of_int <- bn_ofint,
-                                                 op idR <- bn_ofint  0,
-                                                 op ( ** ) <- Int.(+),
-                                                 op ( *** ) <=  fun a b => bn_ofint ((valR a + valR b) %% P)
-proof*.
-realize Rsize_max. smt(). qed.
-realize Rsize_pos. smt(). qed.
-realize valr_pos. smt (@W64x4). qed.
-realize iii.  rewrite /Rbits. 
-progress. rewrite  size_int2bs. auto. qed.
-realize valr_ofint.  progress.
-search bn_ofint.
-rewrite bn_ofintK. smt.
+lemma bn_div2_correct  z :
+  hoare[ M.div2 : arg = (z,2*nlimbs)  ==> (W64x8.valR res) = (W64x8.valR2 z) %/  2^(8*64) ].
+proc. sp.
+while (aux = 2*nlimbs /\ i <= 2*nlimbs /\ forall j, 0 <= j < i => r.[j] = x.[2*nlimbs + j]) . progress. wp. skip. progress.
+smt. smt. skip. progress.
+smt. 
+have ->: 13407807929942597099574024998205846127479365820592393377723561443721764030073546976801874298166903427690031858186486050853753882811946569946433649006084096 = W64x8.M^8. smt.
+have ->: (R2.bnk 16 x{hr})%R2 = valR2 x{hr}. auto.
+rewrite R2.bghint_div. auto.
+rewrite - R.bnkup0.
+rewrite /bnkup.
+have ->: 
+  bigi predT (fun (i1 : int) => to_uint r0.[i1] * W64x8.M ^ (i1 - 0)) 0 8
+  = bigi predT (fun (i1 : int) => to_uint x{hr}.[i1 + 8] * W64x8.M ^ (i1 - 0)) 0 8.
+apply eq_big_int. progress. smt. 
+  have ->: bigi predT (fun (i1 : int) => to_uint x{hr}.[i1] * W64x8.M ^ (i1 - 8)) 8
+  (2 * 8)  = bigi predT (fun (i1 : int) => to_uint x{hr}.[i1] * W64x8.M ^ (i1 - 8)) (0 + 8)
+  (2 * 8). auto.
+rewrite big_addn. simplify. auto.
 qed.
-realize P_pos. smt. qed.
-realize ofint_valr. smt(@W64x4). qed.
-realize rbits_bitsr. 
-progress. rewrite /Rbits. rewrite /bitsR. 
-  have ->: (valR (bn_ofint (bs2int x)))%W64x4 = bs2int x.
-rewrite bn_ofintK. smt. smt. qed.
-realize bitsr_rbits. 
-rewrite /Rbits. rewrite /bitsR.
+
+
+
+
+lemma bn_shrink_correct a  :
+  phoare[ M.bn_shrink : arg = a  ==> W64x4.valR res = W64x8.valR a %% W64x4.modulusR ] = 1%r.
+proc.
+sp.
+while (i <= nlimbs /\ forall j, 0 <= j < i => r.[j]%Array4 = x.[j]%Array8) (nlimbs - i). progress. wp. skip. progress.
+smt. smt. smt. skip. progress.
+progress. 
+smt. smt. 
+have ->: W64x4.modulusR = W64x8.M ^ 4. smt.
+rewrite W64x8.R.bn_mod. auto. 
+rewrite /bnk. 
+apply eq_big_seq. progress. rewrite H1. smt. auto.
+qed.
+
+
+
+lemma bn_expand_correct a  :
+  hoare[ M.bn_expand : arg = a  ==> W64x8.valR res = W64x4.valR a ].
+proc.
+sp. 
+seq 1 : (a = x /\ i = nlimbs /\ forall i, i < nlimbs => r.[i] = x.[i]%Array4).
+while (i <= nlimbs /\ forall j, 0 <= j < i => r.[j] = x.[j]%Array4). wp.  skip. progress.
+smt. smt. skip. progress.
+smt.  smt. smt.
+seq 1 : (a = x /\  (forall j, 0 <= j < nlimbs => r.[j]%Array8 = x.[j]%Array4)
+     /\ (forall j, nlimbs <= j < 2*nlimbs => r.[j] = W64.zero)).    
+while (a = x /\ nlimbs <= i <= 2*nlimbs 
+     /\ (forall j, 0 <= j < nlimbs => r.[j]%Array8 = x.[j]%Array4)
+     /\ (forall j, nlimbs <= j < i => r.[j] = W64.zero) ). wp.  skip. progress.
+smt. smt.
+have z : i{hr} <> j. smt. 
+rewrite - H1. auto.  smt.
+case (j = i{hr}). smt.
 progress.
-rewrite int2bsK. auto. simplify. progress. smt(bnk_cmp).
-have : 0 <= valR  x < W64x4.M ^ nlimbs.
-rewrite /valR. 
-apply (bnk_cmp nlimbs).
-progress. smt.
-smt(@W64x4).
-qed.
-realize exp_prop7. progress. smt. qed.
-realize exp_prop6. progress.
-have ->: (valR (bn_ofint ((valR a + valR b) %% P)) + valR c) %% P
-  = ((valR a + valR ((bn_ofint ((valR b + valR c) %% P)))) %% P). 
-rewrite valr_ofint. smt.
-rewrite valr_ofint. smt.
-print zpcgr.
-search edivz Int.(+).
-rewrite modzDml.
-rewrite modzDmr. smt.
-auto.
-qed.
-realize exp_prop5. progress. 
-rewrite valr_ofint. progress. smt. simplify. 
-rewrite modz_small. smt.
-smt. qed.
-realize mult_valr. progress. smt. qed.
-realize idR_leP. smt. qed.
-
-  
-lemma to_uintP: forall (x y : R), valR (x *** y) = (valR x + valR y) %% P.
-progress. rewrite /( *** ). smt.
-qed.
-
-
-module AddM = {
-  proc ith_bit = M.ith_bit
-  proc swapr   = M.swapr
-  proc opr     =  M.addm
-}.
-
-
-
-lemma ith_bit_lemmaEq :
-      equiv[ MM.ith_bit ~ M.ith_bit : ={arg} ==> ={res}].
-proc.
-seq 2 4 : (={c1, c2,kk}). wp.
-skip. progress.
-have -> : 63 = 2^6 - 1. smt().
-rewrite and_mod. auto. simplify.
-have x:  to_uint (ctr{2} `>>` (of_int 6)%W8) = to_uint ctr{2} %/ 64. smt.
-rewrite to_uint_eq.
-auto.
-rewrite to_uintB. smt.
-rewrite to_uintM_small.  smt.
-rewrite  shr_div_le.
-auto. simplify. smt.
-sim.
-qed.
-
-
-
-
-lemma ith_bit_lemma' :
-      equiv[ M.ith_bit ~ Spec.ith_bit : arg{1}.`1 = arg{2}.`1 /\  W64.to_uint arg{1}.`2 = arg{2}.`2 /\
- 0 <= ctr{2} && ctr{2} < 256 ==>
-              ={res} /\ (res{2} = W64.one \/ res{2} = W64.zero)].
-transitivity MM.ith_bit
-   (={arg} ==> ={res})
-   (arg{1}.`1 = arg{2}.`1 /\  W64.to_uint arg{1}.`2 = arg{2}.`2 /\
- 0 <= ctr{2} && ctr{2} < 256 ==>
-              ={res} /\ (res{2} = W64.one \/ res{2} = W64.zero)).
-progress. smt(). smt().
-symmetry. conseq ith_bit_lemmaEq. auto. auto.
-proc.
-seq 3 0 : (to_uint c1{1} = (to_uint ctr{1} %/ 64) /\ to_uint c2{1} = (to_uint ctr{1} %% 64) /\ to_uint ctr{1} = ctr{2}
-  /\ r{1} = kk{1}.[(to_uint ctr{1} %/ 64)]%Array4 /\ r{2} = kk{1} /\ 0 <= ctr{2} && ctr{2} < 256 ).
-wp.  skip. progress.
+have : j < i{hr}. timeout 10. smt.
+progress.
+rewrite - (H2 j).  smt.
 smt.
-rewrite modzE.
-have <-: to_uint (ctr{1} `>>` (of_int 6)%W8) = to_uint ctr{1} %/ 64. smt.
-rewrite to_uintB.
-smt.
-smt.
-smt.
-exists* r{1}, c2{1}. elim*. progress.
-call {1} (ithbit64 r_L c2_L). skip.
-progress. smt. smt.
-rewrite /ith_bitword64.  rewrite H0.
-rewrite /ith_bitR. rewrite /Rbits. rewrite /valR.
-rewrite /ith_bit.
-rewrite /as_word.
-rewrite /as_w64.
-have ->: (kk{1}.[to_uint ctr{1} %/ 64])%Array4.[to_uint ctr{1} %% 64]
-  = nth false (int2bs 256 ((valR kk{1}))%W64x4) (to_uint ctr{1}) .
-rewrite - get_w2bits.
-rewrite - get_to_list.
-have -> : (W64.w2bits (nth witness ((to_list kk{1}))%Array4 (to_uint ctr{1} %/ 64)))
- = ((nth witness (map W64.w2bits (to_list kk{1}))%Array4 (to_uint ctr{1} %/ 64))).
-rewrite - (nth_map witness witness W64.w2bits). progress.   smt. smt.
-auto.
-have -> : (nth witness (map W64.w2bits ((to_list kk{1}))%Array4)
-     (to_uint ctr{1} %/ 64))
- = (nth [] (map W64.w2bits ((to_list kk{1}))%Array4)
-     (to_uint ctr{1} %/ 64)).
-rewrite (nth_change_dfl [] witness). progress.  smt. smt. auto.
-rewrite - (BitChunking.nth_flatten false 64 (map W64.w2bits ((to_list kk{1}))%Array4) (to_uint ctr{1})).
-rewrite  List.allP. progress. timeout 5.
-have : exists z, z \in ((to_list kk{1}))%Array4 /\ x = W64.w2bits z.
-apply mapP. auto. elim. progress.
-have ->: (flatten (map W64.w2bits ((to_list kk{1}))%Array4))  = (int2bs 256 ((valR kk{1}))%W64x4).
-have -> : (valR kk{1})%W64x4 = bs2int (flatten (map W64.w2bits ((to_list kk{1}))%Array4)).
-rewrite /bnk.
-have ->: range 0 4 = [0;1;2;3].  rewrite range_ltn. auto.
-rewrite range_ltn. auto. rewrite range_ltn. auto.
-simplify. rewrite range_ltn. auto.
-simplify. rewrite range_geq. auto. auto.
-rewrite big_consT.
-rewrite big_consT.
-rewrite big_consT.
-rewrite big_consT.
-rewrite big_nil.
+skip.  progress.
+smt. smt. smt. 
+skip.  progress.
+have -> : valR r{hr} = (bn_seq ((to_list r{hr}))%Array8).
+apply W64x8.R.bn2seq. 
 rewrite /to_list.
-search mkseq.
-print mkseqSr.
-have ->: 4 = 0 + 1 + 1 + 1 + 1 . smt().
-rewrite   mkseqS. auto.
-rewrite   mkseqS. auto.
-rewrite   mkseqS. auto.
-rewrite   mkseqS. auto.
-search mkseq.
-rewrite mkseq0. simplify.
-search flatten.
-rewrite flatten_cons.
-rewrite flatten_cons.
-rewrite flatten_cons.
-rewrite flatten_cons.
-rewrite flatten_nil.
-rewrite cats0.
-rewrite bs2int_cat.
-rewrite bs2int_cat.
-rewrite bs2int_cat. simplify.
-smt.
-have ->: 256 = size (flatten (map W64.w2bits ((to_list kk{1}))%Array4)).
-rewrite /to_list.
-have ->: 4 = 0 + 1 + 1 + 1 + 1 . smt().
-rewrite   mkseqS. auto.
-rewrite   mkseqS. auto.
-rewrite   mkseqS. auto.
-rewrite   mkseqS. auto.
-rewrite mkseq0. simplify.
-rewrite flatten_cons.
-rewrite flatten_cons.
-rewrite flatten_cons.
-rewrite flatten_cons.
-rewrite flatten_nil.
-rewrite size_cat.
-rewrite size_cat.
-rewrite size_cat.
-rewrite size_cat.
+have -> : 8 = 4 + 4. smt().
+rewrite mkseq_add. auto. auto.
+have -> : mkseq (fun (i0 : int) => r{hr}.[i0]) nlimbs 
+  = mkseq (fun (i0 : int) => x{hr}.[i0]%Array4) nlimbs.
+apply eq_in_mkseq. progress. 
+simplify.
+have ->: mkseq (fun (i0 : int) => r{hr}.[nlimbs + i0]) nlimbs
+  = mkseq (fun (i0 : int) => W64.zero) nlimbs.
+apply eq_in_mkseq. progress. rewrite H0. smt. auto.
+rewrite mkseq_nseq. 
+rewrite /bn_seq.
+rewrite foldr_cat.
+have ->: (foldr (fun (w : W64.t) (r0 : int) => to_uint w + W64x8.M * r0) 0
+     (nseq nlimbs W64.zero)) = 0.  
+   have gen : forall n, 0 <= n => foldr (fun (w : W64.t) (r0 : int) => to_uint w + W64x8.M * r0) 0
+                 (nseq n  W64.zero) = 0.
+   apply intind. progress. rewrite nseq0. simplify. auto.
+   progress. rewrite nseqS. auto. search  foldr. simplify. rewrite H2. auto.
+   apply gen. auto.
+rewrite W64x4.R.bn2seq. rewrite /bn_seq. rewrite /to_list. 
+pose f := (fun (w : W64.t) (r0 : int) => to_uint w + W64x8.M * r0).
 simplify. auto.
-rewrite  bs2intK. auto. auto.
-auto. smt().
+qed.
+
+lemma bn_expand_correct_ph a  :
+    phoare[ M.bn_expand : arg = a  ==> W64x8.valR res <> W64x4.valR a ] = 0%r.
+     hoare.
+ conseq (bn_expand_correct a).
+qed.
+
+lemma bn_expand_correct_ph2 a  :
+    phoare[ M.bn_expand : arg = a  ==> W64x8.valR res =  W64x4.valR a ] = 1%r.
+bypr. progress.
+ have ->:  1%r = Pr[M.bn_expand(arg{m}) @ &m : true ] . admit.
+  have ->: Pr[M.bn_expand(arg{m}) @ &m : true]
+  = Pr[M.bn_expand(arg{m}) @ &m : (W64x8.valR res =  W64x4.valR arg{m}) ]  + Pr[M.bn_expand(arg{m}) @ &m : (W64x8.valR res <>  W64x4.valR arg{m}) ].
+rewrite Pr[mu_split (W64x8.valR res =  W64x4.valR arg{m})]. simplify.   auto.
+have ->: Pr[M.bn_expand(arg{m}) @ &m : valR res <> valR arg{m}] = 0%r.
+byphoare (_: arg = arg{m} ==> _). conseq (bn_expand_correct_ph arg{m}). auto. auto. simplify. auto.
 qed.
 
 
 
-
-lemma klo : 
-  equiv[ AddM.opr ~ Spec.mul :
-            ={a} /\ ={b} /\  valR p{1} = P /\ valR a{1} < P /\ valR b{1} < P ==>
-            ={res} /\ valR res{1} < P].
-symmetry.
-transitivity ASpecFp.addm 
-  (ImplFp arg{1}.`1  arg{2}.`1 /\ ImplFp arg{1}.`2  arg{2}.`2 ==> ImplFp res{1} res{2} )
-  (ImplFp a{2} a{1} /\ ImplFp b{2} b{1} /\  valR p{2} = P /\ valR a{2} < P /\ valR b{2} < P ==>
-            ImplFp res{2} res{1} /\ valR res{2} < P).
-    progress. 
-  exists (inzp (valR a{1}), inzp (valR b{1}) )%W64x4. progress.
-rewrite inzpK. rewrite modz_small. smt. smt.
-rewrite inzpK. rewrite modz_small. smt. smt.
-rewrite inzpK. rewrite modz_small. smt. smt.
-rewrite inzpK. rewrite modz_small. smt. smt.
-progress. smt. 
-proc.  wp. skip.  progress.
-rewrite to_uintP.
-       rewrite H H0.
-     rewrite addE.
-auto.
-symmetry. 
-transitivity M.addm 
-  (arg{1}.`1 = arg{2}.`1 /\ arg{1}.`2 = arg{2}.`2 /\ arg{1}.`3 = arg{2}.`3 ==> ={res})   
-  (ImplZZ p{1} P /\ ImplFp arg{1}.`2  arg{2}.`1 /\ ImplFp arg{1}.`3  arg{2}.`2 ==> ImplFp res{1} res{2} /\ valR res{1} < P ).
-progress.  exists (p{1},a{1},b{1}). progress. progress. 
-proc*.  sim.
-conseq addm_spec. progress. smt.
-qed.
-
-
-lemma ones64 : (2^64  - 1)  = 18446744073709551615. smt(). qed.
-
-lemma swap_lemma :
-      equiv[ AddM.swapr ~ Spec.swapr :
-              a{2} = x{1} /\ b{2} = y{1} /\ swap_0{1} = as_w64 c{2} ==> ={res}].
-proc.  simplify.
-seq 2 0 : (i{1} = 0 /\ a{2} = x{1} /\ b{2} = y{1} /\ swap_0{1} = as_w64 c{2} /\ 
-   ((as_bool swap_0{1} => mask{1} = (of_int 18446744073709551615)%W64 )
-              /\ (as_bool swap_0{1} = false => mask{1} = (of_int 0)%W64))).
-wp. skip. progress. smt(@W64). smt.
-while {1} (0 <= i{1} /\ ((as_bool swap_0{1} => mask{1} = (of_int 18446744073709551615)%W64 )
-              /\ (as_bool swap_0{1} = false => mask{1} = (of_int 0)%W64)) 
-   /\ (forall j, 0 <= j < i{1} => (x{1}.[j])%Array4 = (if as_bool swap_0{1} then (b{2}.[j]) else (a{2}.[j]))%Array4 )  
-   /\ (forall j, 0 <= j < i{1} => (y{1}.[j])%Array4 = (if as_bool swap_0{1} then (a{2}.[j]) else (b{2}.[j]))%Array4 )  
-   /\ (forall j, i{1} <= j => (x{1}.[j])%Array4 =  (a{2}.[j]))%Array4
-   /\ (forall j, i{1} <= j => (y{1}.[j])%Array4 =  (b{2}.[j]))%Array4
- ) (nlimbs - i{1} + 1).
-progress. wp.  skip.  progress.   smt().
-case (j <  i{hr}). progress.  timeout 15. smt.
-progress.
-have : j = i{hr}. smt.
-progress.
-have ->: (x{hr}.[i{hr} <-
-    x{hr}.[i{hr}] `^` (x{hr}.[i{hr}] `^` y{hr}.[i{hr}] `&` mask{hr})].[i{hr}])%Array4
- = (x{hr}.[i{hr}] `^` (x{hr}.[i{hr}] `^` y{hr}.[i{hr}] `&` mask{hr}))%Array4. smt.
-case (as_bool swap_0{hr}). progress.
-rewrite H4. auto.  rewrite H0. auto. rewrite H5. auto. rewrite - ones64. 
-have -> : ((a{m}.[i{hr}])%Array4 `^` (b{m}.[i{hr}])%Array4 `&`
- (of_int W64.max_uint)%W64) = a{m}.[i{hr}]%Array4 `^` ((b{m}.[i{hr}])%Array4 `&`
- (of_int W64.max_uint)%W64). smt. 
-have ->: ((b{m}.[i{hr}])%Array4 `&` (of_int W64.max_uint)%W64) = ((b{m}.[i{hr}])%Array4). smt.
-smt(@W64).
-progress. rewrite H4. auto.  rewrite H1. smt(). auto. 
-case (j <  i{hr}). progress.  timeout 15. smt.
-progress.
-have : j = i{hr}. smt.
-progress.
-have ->: (y{hr}.[i{hr} <-
-   y{hr}.[i{hr}] `^` (x{hr}.[i{hr}] `^` y{hr}.[i{hr}] `&` mask{hr})].[i{hr}])%Array4
- = (y{hr}.[i{hr}] `^` (x{hr}.[i{hr}] `^` y{hr}.[i{hr}] `&` mask{hr}))%Array4. smt.
-case (as_bool swap_0{hr}). progress.
-rewrite H4. auto.  rewrite H0. auto. rewrite H5. auto. rewrite - ones64. 
-have -> : ((a{m}.[i{hr}])%Array4 `^` (b{m}.[i{hr}])%Array4 `&`
- (of_int W64.max_uint)%W64) = a{m}.[i{hr}]%Array4 `^` ((b{m}.[i{hr}])%Array4 `&`
- (of_int W64.max_uint)%W64). smt. 
-have ->: ((b{m}.[i{hr}])%Array4 `&` (of_int W64.max_uint)%W64) = ((b{m}.[i{hr}])%Array4). smt.
-smt(@W64).
-progress. rewrite H4. auto.  rewrite H1. smt(). smt(@W64).
-smt. smt. smt.
-skip. progress. smt().   smt().   smt(). 
-case (c{2} = false). progress.  
-apply Array4.ext_eq.  progress. rewrite H5. progress. smt(). rewrite /as_bool. rewrite /as_w64. simplify. smt(@W64).
-apply Array4.ext_eq.  progress. rewrite H6. progress. smt(). rewrite /as_bool. rewrite /as_w64. simplify. smt(@W64).
-progress. have ->: c{2} = true. smt(). simplify.
-progress. 
-apply Array4.ext_eq.  progress. rewrite H5. progress. smt(). rewrite /as_bool. rewrite /as_w64. simplify. smt(@W64).
-apply Array4.ext_eq.  progress. rewrite H6. progress. smt(). rewrite /as_bool. rewrite /as_w64. simplify. smt(@W64).
-qed.
-
-
-
-lemma mulm_real_spec : 
-      equiv[ M1.iterop_spec ~ M7(AddM).iterop :
-            ImplZZ m{2} P /\
-            ={x} /\
-            bs2int n{1} = valR n{2} /\ size n{1} = 256 /\ valR x{1} < P ==>
-            ={res}].
-apply (iterop_real_speac AddM _ _ _). conseq swap_lemma. smt(). smt().
-conseq ith_bit_lemma'. smt().
-conseq klo. smt(). auto. auto.
-qed.
-
-
-
-lemma right_end : 
- equiv[ M7(AddM).iterop ~ M.mulm : ={arg} ==> ={res} ].
-proc. sim.
-seq  7  22 : (={x1,x2,x3,x4,d,ctr,n,m}). sim. wp. 
-call (_:true). sim. wp.  call (_:true). sim. wp.  skip. progress. apply ext_eq_all. auto. rewrite /oneR. 
-have x : valR%W64x4 (witness.[0 <- W64.zero].[1 <- W64.zero].[2 <- W64.zero].[3 <- W64.zero])%Array4 = 0.
-progress. rewrite /bnk.
-have ->: range 0 4 = [0;1;2;3].  rewrite range_ltn. auto.
-rewrite range_ltn. auto. rewrite range_ltn. auto. 
-simplify. rewrite range_ltn. auto. 
-simplify. rewrite range_geq. auto. auto.
-rewrite big_consT.
-rewrite big_consT.
-rewrite big_consT.
-rewrite big_consT. 
-rewrite big_nil.
-simplify. auto.
-smt.
-have x : valR%W64x4 (witness.[0 <- W64.zero].[1 <- W64.zero].[2 <- W64.zero].[3 <- W64.zero])%Array4 = 0.
-progress. rewrite /bnk.
-have ->: range 0 4 = [0;1;2;3].  rewrite range_ltn. auto.
-rewrite range_ltn. auto. rewrite range_ltn. auto. 
-simplify. rewrite range_ltn. auto. 
-simplify. rewrite range_geq. auto. auto.
-rewrite big_consT.
-rewrite big_consT.
-rewrite big_consT.
-rewrite big_consT. 
-rewrite big_nil.
-simplify. auto.
-smt.
-while (={x1,x2,x3,x4,d,ctr,n,m}). wp.
-call (_:true). sim. wp. 
-call (_:true). sim. wp. 
-call (_:true). sim. 
-call (_:true). sim. 
-call (_:true). sim. 
-wp.
-call (_:true). sim. 
-call (_:true). sim. 
-wp. skip. progress.
-smt(@W64).
-skip. progress.
-qed.
-
-
-
-
-lemma kk :  forall (n : int), 0 <= n => forall (a : zp) (b : R.t), valR%W64x4 b < P =>
-  ImplFp b a =>
-  ImplFp (Mult.(^) b n) (inzp (asint a * n)).
-apply intind. progress.
-rewrite exp_prop1.
-smt.
-(* have -> : (Sub.val (inzp 1))%Sub = 1. smt. *)
-(* smt(valR_one). *)
-progress.
-have ->: (Mult.(^) b (i + 1)) = b *** (Mult.(^) b  i).
-rewrite exp_prop3. auto. auto.  auto.
-rewrite exp_prop2.
-rewrite exp_prop7. smt.
-have ->:  (asint a * (i + 1)) =   (asint a + (asint a * i)).
-smt().
-have ->:  inzp (asint a + (asint a * i)) = (inzp (asint a)) + (inzp (asint a * i)).
-smt.
-rewrite - H2. 
-print ImplFp.
-have ->: asint (inzp (valR b) + inzp (valR b * i))
-  = (asint (inzp (valR%W64x4 b)) + (asint  (inzp (valR%W64x4 b * i)))) %% P.
-smt.
-have ih :  ImplFp (b ^ i)%Mult  (inzp (valR%W64x4 b * i)).
-smt.
- (* apply H0. auto. auto. *)
-rewrite - ih.
-have ->: asint (inzp (valR%W64x4 b)) = valR%W64x4 b. smt.
-simplify. 
-rewrite  to_uintP /=. done.
-qed.
-
-
-
-
-lemma left_end :
- equiv[ ASpecFp.mulm ~ M1.iterop_spec  :
-    ImplFp arg{2}.`1 arg{1}.`1 /\  bs2int arg{2}.`2  = asint arg{1}.`2 /\ valR%W64x4 x{2} < P ==> ImplFp res{2} res{1}].
-proc.
-wp.  skip.  progress.
-rewrite  (kk (bs2int n{2}) _ a{1}). smt. auto. auto. smt.
-qed.
-
-
-
-
-
-
-equiv mulm_spec:
- M.mulm ~ ASpecFp.mulm:
-  valR m{1} = P /\ ImplFp x{1} a{2} /\ ImplFp n{1} b{2} /\ ImplZZ m{1} P ==> ImplFp res{1} res{2}.
-proof. symmetry.
-transitivity M1.iterop_spec
-  (ImplFp arg{2}.`1 arg{1}.`1 /\  bs2int arg{2}.`2  = asint arg{1}.`2 /\ valR%W64x4 x{2} < P ==> ImplFp res{2} res{1})
-  ( valR%W64x4 m{2} = P /\
-            ={x} /\
-            bs2int n{1} = valR%W64x4 n{2} /\ (size n{1}) = 256 /\ valR%W64x4 x{1} < P ==>
-            ={res}).
-progress. exists (x{2},Rbits n{2}).
-progress. 
-rewrite /Rbits. smt.
-smt.
-rewrite /Rbits. smt.
-rewrite /Rbits. smt.
-smt.
-auto.
-conseq left_end. 
-symmetry.
-transitivity M7(AddM).iterop
- (={arg} ==> ={res})
- (  valR%W64x4 m{1} = P /\
-  x{2} = x{1} /\ bs2int n{2} = valR%W64x4 n{1} /\ size n{2} = 256 /\ valR%W64x4 x{2} < P ==> ={res}).
-progress. smt(). smt().
-symmetry.
-conseq right_end.
-auto. auto. 
-symmetry.
-conseq mulm_real_spec.
-progress. 
-qed.
-
-
-
-
-clone import Abstract_exp_proof_8 as Exp with type R  <- R.t,
-                                                 op P <- P,
-                                                 op Rsize <- 256,
-                                                 op valR <- W64x4.valR,
-                                                 op of_int <- bn_ofint,
-                                                 op idR <- bn_ofint 1,
-                                                 op ( ** ) <- Int.( * ),
-                                                 op ( *** ) <=  fun a b => bn_ofint ((valR a * valR b) %% P)
-proof*.
-realize Rsize_max. smt(). qed.
-realize Rsize_pos. smt(). qed.
-realize valr_pos. smt (@W64x4). qed.
-realize iii.  rewrite /Rbits. 
-progress. rewrite  size_int2bs. auto. qed.
-realize valr_ofint.  progress.
-search bn_ofint.
-rewrite bn_ofintK. smt.
-qed.
-realize P_pos. smt. qed.
-realize ofint_valr. smt(@W64x4). qed.
-realize rbits_bitsr. 
-progress. rewrite /Rbits. rewrite /bitsR. 
-  have ->: (valR (bn_ofint (bs2int x)))%W64x4 = bs2int x.
-rewrite bn_ofintK. smt. smt. qed.
-realize bitsr_rbits. 
-rewrite /Rbits. rewrite /bitsR.
-progress.
-rewrite int2bsK. auto. simplify. progress. smt(bnk_cmp).
-have : 0 <= valR  x < W64x4.M ^ nlimbs.
-rewrite /valR. 
-apply (bnk_cmp nlimbs).
-progress. smt.
-smt(@W64x4).
-qed.
-realize exp_prop7. progress. smt. qed.
-realize exp_prop6. progress.
-have ->: (valR (bn_ofint ((valR a * valR b) %% P)) * valR c) %% P
-  = ((valR a * valR ((bn_ofint ((valR b * valR c) %% P)))) %% P). 
-rewrite valr_ofint. smt.
-rewrite valr_ofint. smt.
-rewrite modzMml.
-rewrite modzMmr. smt.
-auto.
-qed.
-realize exp_prop5. progress. 
-rewrite valr_ofint. progress. smt. simplify. 
-rewrite modz_small. smt.
-smt. qed.
-realize mult_valr. progress. smt. qed.
-realize idR_leP. smt. qed.
-
-  
-
-module MultM = {
-  proc ith_bit = M.ith_bit
-  proc swapr   = M.swapr
-  proc opr     =  M.mulm
-}.
-
-
-lemma okl : 
-  equiv[ MultM.opr ~ Exp.Spec.mul :
-            x{1} = a{2} /\ n{1} = b{2} /\  valR m{1} = P /\ valR x{1} < P /\ valR n{1} < P ==>
-            ={res} /\ valR res{1} < P].
-symmetry.
-transitivity ASpecFp.mulm 
-  (ImplFp arg{1}.`1  arg{2}.`1 /\ ImplFp arg{1}.`2  arg{2}.`2 ==> ImplFp res{1} res{2} )
-  (ImplFp x{2} a{1} /\ ImplFp n{2} b{1} /\  valR m{2} = P /\ valR x{2} < P /\ valR n{2} < P ==>
-            ImplFp res{2} res{1} /\ valR res{2} < P).
-    progress. 
-  exists (inzp (valR a{1}), inzp (valR b{1}) )%W64x4. progress.
-rewrite inzpK. rewrite modz_small. smt. smt.
-rewrite inzpK. rewrite modz_small. smt. smt.
-rewrite inzpK. rewrite modz_small. smt. smt.
-rewrite inzpK. rewrite modz_small. smt. smt.
-progress. smt. 
-proc.  wp. skip.  progress.
-       rewrite H H0.
-smt.
-auto.
-symmetry. 
-conseq mulm_spec. progress. smt.
-qed.
-
-
-
-
-lemma expm_real_spec : 
-      equiv[ Exp.M1.iterop_spec ~ Exp.M7(MultM).iterop :
-            ImplZZ m{2} P /\
-            ={x} /\
-            bs2int n{1} = valR n{2} /\ size n{1} = 256 /\ valR x{1} < P ==>
-            ={res}].
-apply (Exp.iterop_real_speac MultM _ _ _). 
-
-transitivity M.swapr
-  (={arg} ==> ={res})
-  (a{2} = x{1} /\ b{2} = y{1} /\ swap_0{1} = (as_w64 c{2})%Mult ==>
-          ={res}).
-progress. smt(). smt().
-proc. sim.
-
-symmetry.
-transitivity Mult.Spec.swapr
-  (={arg} ==> ={res})
-  (a{1} = x{2} /\ b{1} = y{2} /\ swap_0{2} = (as_w64 c{1})%Mult ==>
-          ={res}).
-smt(). smt().
-proc. sim.
-
-symmetry. conseq swap_lemma. smt(). 
-
-transitivity MultM.ith_bit
-  (={arg} ==> ={res})
-  (arg{1}.`1 = arg{2}.`1 /\ ImplWord ctr{1} ctr{2} /\ 0 <= ctr{2} && ctr{2} < 256 ==>
-          ={res} /\ (res{2} = W64.one \/ res{2} = W64.zero)).
-smt(). smt().
-proc. sim.
-        
-
-
-symmetry.
-transitivity Mult.Spec.ith_bit
-  (={arg} ==> ={res})
-  (arg{1}.`1 = arg{2}.`1 /\ ImplWord ctr{2} ctr{1} /\ 0 <= ctr{1} && ctr{1} < 256 ==>
-          ={res} /\ (res{2} = W64.one \/ res{2} = W64.zero)).
-smt(). smt().
-
-
-proc.  skip.  auto.
-
-symmetry.
-conseq ith_bit_lemma'. progress.  smt(). smt().
-conseq okl. smt(). auto. auto.
+    
+equiv bnreduce_spec:
+ M.bnreduce ~ CSpecFp.redm:
+     W64x8.valR a{1} = a{2} 
+ /\  W64x8.valR r{1} = r{2} 
+ /\  W64x4.valR p{1} = P
+ /\  k{2} = nlimbs
+   ==>  (W64x4.valR res{1}) = res{2}  %% W64x4.modulusR.
+proof. proc.
+sp.
+simplify.
+seq 0 0 : (valR a{1} = a{2} /\ valR r{1} = r{2} /\ ImplZZ p{1} P /\ k{2} = nlimbs). skip. auto.
+seq 1 1 : (valR a{1} = a{2} /\ valR r{1} = r{2} /\ ImplZZ p{1} P /\ k{2} = nlimbs
+    /\ W64x8.valR2 xr{1} = xr{2} (* /\ xr{2} = a{2} * r{2} *)).
+call dmuln_spec. skip. progress.
+seq 1 1 : (valR a{1} = a{2} /\ valR r{1} = r{2} /\ ImplZZ p{1} P /\ k{2} = nlimbs
+    /\ W64x8.valR2 xr{1} = xr{2} /\ W64x4.valR xrf{1} = xrf{2} ).
+admit.
+(* ecall {1} (bn_div2_correct xr{1} (2 * nlimbs)). inline*. wp.  skip.  progress. *)
+inline ASpecFp.div2.
+seq 1 1 : (valR a{1} = a{2} /\ valR r{1} = r{2} /\ ImplZZ p{1} P /\ k{2} = nlimbs
+    /\ W64x8.valR2 xr{1} = xr{2} /\ W64x4.valR xrf{1} = xrf{2} 
+    /\  W64x8.valR xrfn{1} = xrfn{2}).
+call muln_spec. skip. progress.
+seq 1 1 : (valR a{1} = a{2} /\ valR r{1} = r{2} /\ ImplZZ p{1} P /\ k{2} = nlimbs
+    /\ W64x8.valR2 xr{1} = xr{2} /\ W64x4.valR xrf{1} = xrf{2} 
+    /\ W64x8.valR xrfn{1} = xrfn{2}
+    /\ W64x8.valR t{1} = t{2}).
+call dsubc_spec. skip. progress.
+seq 1 0 : (valR a{1} = a{2} /\ valR r{1} = r{2} /\ ImplZZ p{1} P /\ k{2} = nlimbs
+    /\ W64x8.valR2 xr{1} = xr{2} /\ W64x4.valR xrf{1} = xrf{2} 
+    /\ W64x8.valR xrfn{1} = xrfn{2}
+    /\ W64x8.valR t{1} = t{2}
+    /\ W64x8.valR pp{1} = W64x4.valR p{1}).
+ecall {1} (bn_expand_correct_ph2 p{1} ). skip. progress.
+seq 1 1 : (valR a{1} = a{2} /\ valR r{1} = r{2} /\ ImplZZ p{1} P /\ k{2} = nlimbs
+    /\ W64x8.valR2 xr{1} = xr{2} /\ W64x4.valR xrf{1} = xrf{2} 
+    /\ W64x8.valR xrfn{1} = xrfn{2}
+    /\ W64x8.valR t{1} = t{2}
+    /\ W64x8.valR pp{1} = W64x4.valR p{1}
+    /\ W64x8.valR t{1} = t{2} ).
+call dcminusP_spec. skip. progress. smt().
+seq 1 0 : (valR a{1} = a{2} /\ valR r{1} = r{2} /\ ImplZZ p{1} P /\ k{2} = nlimbs
+    /\ W64x8.valR2 xr{1} = xr{2} /\ W64x4.valR xrf{1} = xrf{2} 
+    /\ W64x8.valR xrfn{1} = xrfn{2}
+    /\ W64x8.valR t{1} = t{2}
+    /\ W64x8.valR pp{1} = W64x4.valR p{1}
+    /\ W64x8.valR t{1} = t{2}
+    /\ W64x4.valR res_0{1} = W64x8.valR t{1} %% W64x4.modulusR).
+ecall {1} (bn_shrink_correct t{1}). skip. progress.
+skip.  progress. 
 qed.
 
 
