w64x4/proof/Fp_w64x4_spec.ec
@@ -5,7 +5,7 @@ import Ring.IntID IntOrder.
 require import JModel.
 require import JBigNum.
 
-require import Array4 Array8.
+require import Array4 Array8 Array16.
 
 abbrev nlimbs = 4.
 
@@ -15,17 +15,24 @@ clone import BigNum as W64x4 with
  theory R2.A <= Array8
  proof gt0_nlimbs by done.
 
+
+clone import BigNum as W64x8 with
+ op nlimbs <- 8,
+ theory R.A <= Array8,
+ theory R2.A <= Array16
+ proof gt0_nlimbs by done.
+
+ 
 type R = W64.t Array4.t.
 type R2 = W64.t Array8.t.
 
 abbrev M = 115792089237316195423570985008687907853269984665640564039457584007913129639936.
-(* modular operations modulo P *)
 
 
 op P : int. 
 
 axiom P_prime: prime P.
-axiom ppos : 2 * P < M.
+axiom ppos : 2 * P < W64x4.modulusR.
 
 
 (* Embedding into ring theory *)
@@ -38,26 +45,26 @@ clone import ZModP.ZModField as Zp with
         
 (** "Implements" relation *)
 abbrev ImplWord x y = W64.to_uint x = y.
-abbrev ImplZZ x y = valR x = y.
-abbrev ImplZZ2 x y = valR2 x = y.
-abbrev ImplFp x y = valR x = asint y.
+abbrev ImplZZ x y = W64x4.valR x = y.
+abbrev ImplZZ2 x y = W64x4.valR2 x = y.
+abbrev ImplFp x y = W64x4.valR x = asint y.
 
 
 op pR: R.
 axiom pRE: ImplZZ pR P.
 
-op zeroR : R = R.A.of_list W64.zero
+op zeroR : R = W64x4.R.A.of_list W64.zero
                  [ W64.zero; W64.zero; W64.zero; W64.zero ].
 
 
 
 lemma zeroRE: valR zeroR = 0.
 proof.
-by rewrite /zeroR R.bn2seq /= R.A.of_listK 1:/# /bn_seq.
+by rewrite /zeroR W64x4.R.bn2seq /= W64x4.R.A.of_listK 1:/# /bn_seq.
 qed.
 
 
-op (^) (x : zp)(n : R.t) : zp = inzp (asint x ^ W64x4.valR n).
+op (^) (x : zp)(n : W64x4.R.t) : zp = inzp (asint x ^ W64x4.valR n).
 
 
 (******************************************************************)
@@ -68,8 +75,8 @@ module ASpecFp = {
   (* INTEGER OPS *)
   proc addn(a b: int): bool * int = {
     var c, r;
-    c <- modulusR <= (a+b);
-    r <- (a + b) %% modulusR;
+    c <- W64x4.modulusR <= (a+b);
+    r <- (a + b) %% W64x4.modulusR;
     return (c, r);
   }
   proc muln(a b: int): int = {
@@ -77,19 +84,37 @@ module ASpecFp = {
     r <- a * b;
     return r;
   }
+ proc redm(a: int): int = {
+   var r;
+   r <- a %% P;
+  return r;
+ }
+ proc div2(a, n: int): int = {
+   var r;
+   r <- a %/  (2 ^ n);
+  return r;
+ }
 
-  proc subn(a b: int): bool * int = {
+  (* proc subn(a b: int): bool * int = { *)
+  (*   var c, r; *)
+  (*   c <- a < b; *)
+  (*   r <- (a - b) %% W64x4.modulusR; *)
+  (*   return (c, r); *)
+  (* }   *)
+
+  proc dsubn(a b: int): bool * int = {
     var c, r;
     c <- a < b;
-    r <- (a - b) %% modulusR;
+    r <- (a - b) %% W64x8.modulusR;
     return (c, r);
-  }  
+  }
+  
   proc ctseln(cond: bool, c a: int): int = {
     var r;
     r <- (if cond then a else c);
     return r;
   }
-  proc cminusP(a: int): int = {
+  proc cminusP(a : int): int = {
     var r;
     r <- if a < P then a else a-P;
     return r;
@@ -109,18 +134,13 @@ module ASpecFp = {
     r <- Zp.zero;
     return r;
   }
-  (* modular operations: finite field [Fp] *)
-  proc addm(a b: zp): zp = {
-    var r;
-    r <- a + b;
-    return r;
-  }
+
   proc mulm(a b: zp): zp = {
     var r;
     r <- a * b;
     return r;
   }
-  proc expm(a : zp,  b: R.t): zp = {
+  proc expm(a : zp,  b: W64x4.R.t): zp = {
     var r;
     r <- a ^ b;
     return r;
@@ -128,42 +148,73 @@ module ASpecFp = {
   
 }.
 
-
+require import IntDiv.
 module CSpecFp = {
- proc addm(a b: zp): int = {
-  var c, x, r;
-  (c, x) <@ ASpecFp.addn(asint a, asint b);
-  r <@ ASpecFp.cminusP(x);
-  return r;
+
+ proc redm(a r k: int): int = {
+   var xr, xrf, xrfn, t, b;
+  xr    <@ ASpecFp.muln(a,r);
+  xrf   <@ ASpecFp.div2(xr, 2*k);
+  xrfn  <@ ASpecFp.muln(xrf, P);
+  (b,t) <@ ASpecFp.dsubn(a, xrfn);
+  t     <@ ASpecFp.cminusP(t);
+  return t;
  }
- proc cminusP(a: int): int = {
+
+
+ proc dcminusP(a: int): int = {
   var c, x, r;
-  (c, x) <@ ASpecFp.subn(a, P);
+  (c, x) <@ ASpecFp.dsubn(a, P);
   r <@ ASpecFp.ctseln(c, x, a);
   return r;
  }
 
 }.
 
+
 equiv cminusP_eq:
- ASpecFp.cminusP ~ CSpecFp.cminusP: ={a} /\ a{2}<modulusR ==> ={res}.
+ ASpecFp.cminusP ~ CSpecFp.dcminusP: ={arg} /\ a{2}<W64x8.modulusR  ==> ={res}.
 proof.
 proc; inline*; wp; skip => &1 &2.
-have ->: modulusR = 2^256 by rewrite R.bn_modulusE /= !mulrA expr0. 
+have ->: W64x8.modulusR = 2^512 by rewrite W64x8.R.bn_modulusE /= !mulrA expr0.
 progress. smt.
-qed.
-
-equiv addm_eq:
- ASpecFp.addm ~ CSpecFp.addm: ={a,b} ==> asint res{1}=res{2}.
-proof.
-proc; simplify.
-+ inline*; wp; skip => /> &2.
-  have ->: (asint a{2} + asint b{2}) %% modulusR = (asint a{2} + asint b{2}).
-   rewrite modz_small. progress. smt. smt.
-   done.
-  case: (asint a{2} + asint b{2} < P) => H.
-   by rewrite addE modz_small; smt(rg_asint).
-  rewrite addE. smt. 
+(* case (a{2} < P). auto. progress. *)
+(* have : (a{2} - P) < modulusR.  smt. progress. smt. *)
 qed.
 
 
+require import BarrettRedInt.
+require import Real.
+equiv redm_eq:
+ ASpecFp.redm ~ CSpecFp.redm: ={a} /\ r{2} = (nlimbs ^ k{2} %/ P) 
+  /\ 0 < P < W64x4.modulusR
+  /\ 0 <= a{2} < P * P
+  /\ 0 < P < 2 ^ k{2} 
+  /\ 0 <= k{2} ==> ={res}.
+proc. inline*. wp. skip. progress.
+rewrite -  (barrett_reduction_correct a{2} P k{2} ). auto. auto.  auto. 
+rewrite /barrett_reduction. simplify. rewrite /ti. rewrite /ti'. rewrite /ri.
+have ->: 2 ^ (2 * k{2}) = 4 ^ k{2}. smt.
+have <-:  a{2} - a{2} * (nlimbs ^ k{2} %/ P) %/ nlimbs ^ k{2} * P
+ = (a{2} - a{2} * (nlimbs ^ k{2} %/ P) %/ nlimbs ^ k{2} * P) %% W64x4.modulusR2.
+rewrite modz_small.
+
+have -> : a{2} - a{2} * (nlimbs ^ k{2} %/ P) %/ nlimbs ^ k{2} * P
+ = ti a{2} P k{2}. rewrite /ti. rewrite /ti'. rewrite /ri. auto.
+split. 
+   have : 0%r <= (ti a{2} P k{2})%r < 2%r * P%r.
+   rewrite - same_t. auto. auto.
+     apply (st8 a{2}%r P%r k{2}%r _ _). split.  smt. smt. smt.
+  progress. smt. 
+move => _.
+have ->: `|W64x4.modulusR2| = W64x4.modulusR2. smt.
+   have : 0%r <= (ti a{2} P k{2})%r < 2%r * P%r.
+   rewrite - same_t. auto. auto. 
+     apply (st8 a{2}%r P%r k{2}%r _ _). smt.
+split. smt. move => ?. timeout 10. smt.
+  progress.   
+   have : 2 * P < W64x4.modulusR2.   timeout 15. smt.
+smt.
+auto.
+auto.
+qed.
